rewrite: deduction theorem, soundness theorem

src/FOL/deduction.lean
@@ -17,31 +17,26 @@ def eq_axiom4_aux {n} (f : L.fn n) : subformula L 0 (bit0 n) :=
 (⋀ i, #i.bit0 =' #i.bit1) ⟶ (function f (var ∘ fin.bit0) =' function f (var ∘ fin.bit1))
 
 def eq_axiom4 {n} (f : L.fn n) : subformula L 0 0 :=
-(∀'*(eq_axiom4_aux f) : subformula L 0 0)
-
-def eq_axiom5_aux {n} (r : L.pr n) : subformula L 0 (bit0 n) :=
-(⋀ i, #i.bit0 =' #i.bit1) ⟶ relation r (var ∘ fin.bit0) ⟶ relation r (var ∘ fin.bit1)
+∀'*((⋀ i, #i.bit0 =' #i.bit1) ⟶ (function f (var ∘ fin.bit0) =' function f (var ∘ fin.bit1)) : subformula L 0 (bit0 n))
 
 def eq_axiom5 {n} (r : L.pr n) : subformula L 0 0 :=
-(∀'*(eq_axiom5_aux r) : subformula L 0 0)
+∀'*((⋀ i, #i.bit0 =' #i.bit1) ⟶ relation r (var ∘ fin.bit0) ⟶ relation r (var ∘ fin.bit1))
 
 inductive proof : Π {m}, preTheory L m → subformula L m 0 → Type u
-| generalize      {m} {T : preTheory L m} : ∀ {p : subformula L (m + 1) 0},
-    proof T.mlift p → proof T (∀'p.pull)
-| mdp             {m} {T : preTheory L m} : ∀ {p q}, proof T (p ⟶ q) → proof T p → proof T q
-| by_axiom        {m} {T : preTheory L m} : ∀ {p}, p ∈ T → proof T p
-| verum           {m} {T : preTheory L m} : proof T ⊤
-| imply₁          {m} {T : preTheory L m} : ∀ {p q}, proof T (p ⟶ q ⟶ p)
-| imply₂          {m} {T : preTheory L m} : ∀ {p q r}, proof T ((p ⟶ q ⟶ r) ⟶ (p ⟶ q) ⟶ p ⟶ r)
-| contraposition  {m} {T : preTheory L m} : ∀ {p q}, proof T ((∼p ⟶ ∼q) ⟶ q ⟶ p)
-| specialize      {m} {T : preTheory L m} : ∀ {p : subformula L m 1} {t : subterm L m 0},
-    proof T (∀'p ⟶ subst t (push p))
-| univ_K          {m} {T : preTheory L m} : ∀ {p q}, proof T (∀'(p ⟶ q) ⟶ ∀'p ⟶ ∀'q)
-| eq_reflexivity  {T : Theory L} : proof T ∀'(#0 =' #0)
-| eq_symmetry     {T : Theory L} : proof T ∀' ∀'((#0 =' #1) ⟶ (#1 =' #0))
-| eq_transitivity {T : Theory L} : proof T ∀' ∀' ∀'((#0 =' #1) ⟶ (#1 =' #2) ⟶ (#0 =' #2))
-| function_ext    {T : Theory L} : ∀ {n} {f : L.fn n}, proof T (∀'*(eq_axiom4_aux f))
-| predicate_ext   {T : Theory L} : ∀ {n} {r : L.pr n}, proof T (∀'*(eq_axiom5_aux r))
+| generalize   {m} {T : preTheory L m} : ∀ {p}, proof T.mlift p → proof T (∀'p.pull)
+| mdp          {m} {T : preTheory L m} : ∀ {p q}, proof T (p ⟶ q) → proof T p → proof T q
+| by_axiom     {m} {T : preTheory L m} : ∀ {p}, p ∈ T → proof T p
+| verum        {m} {T : preTheory L m} : proof T ⊤
+| imply₁       {m} {T : preTheory L m} : ∀ {p q}, proof T (p ⟶ q ⟶ p)
+| imply₂       {m} {T : preTheory L m} : ∀ {p q r}, proof T ((p ⟶ q ⟶ r) ⟶ (p ⟶ q) ⟶ p ⟶ r)
+| contra       {m} {T : preTheory L m} : ∀ {p q}, proof T ((∼p ⟶ ∼q) ⟶ q ⟶ p)
+| specialize   {m} {T : preTheory L m} : ∀ {p} {t}, proof T (∀'p ⟶ subst t p)
+| dummy_univ   {m} {T : preTheory L m} : ∀ {p q}, proof T (∀'(dummy p ⟶ q) ⟶ p ⟶ ∀'q)
+| eq_refl      {T : Theory L} : proof T ∀'(#0 =' #0)
+| eq_symm      {T : Theory L} : proof T ∀' ∀'((#0 =' #1) ⟶ (#1 =' #0))
+| eq_trans     {T : Theory L} : proof T ∀' ∀' ∀'((#0 =' #1) ⟶ (#1 =' #2) ⟶ (#0 =' #2))
+| function_ext {T : Theory L} : ∀ {n} {f : L.fn n}, proof T (eq_axiom4 f)
+| relation_ext {T : Theory L} : ∀ {n} {r : L.pr n}, proof T (eq_axiom5 r)
 
 instance (m : ℕ) : has_Longarrow (formula L m) := ⟨proof⟩
 
@@ -53,7 +48,7 @@ instance (m) : axiomatic_classical_logic' (formula L m) :=
   { modus_ponens := λ p q ⟨bpq⟩ ⟨bp⟩, ⟨bpq.mdp bp⟩,
     imply₁ := λ p q, ⟨proof.imply₁⟩, 
     imply₂ := λ p q r, ⟨proof.imply₂⟩,
-    contraposition := λ p q, ⟨proof.contraposition⟩,
+    contraposition := λ p q, ⟨proof.contra⟩,
     provable_top := ⟨proof.verum⟩,
     bot_eq := by refl,
     and_def := λ p q, rfl,
@@ -77,1179 +72,179 @@ begin
   { intros U ss, exact verum },
   { intros U ss, exact imply₁ },
   { intros U ss, exact imply₂ },
-  { intros U ss, exact contraposition },
+  { intros U ss, exact contra },
   { intros U ss, exact specialize },
-  { intros U ss, exact univ_K },
-  { intros U ss, exact eq_reflexivity },
-  { intros U ss, exact eq_symmetry },
-  { intros U ss, exact eq_transitivity },
+  { intros U ss, exact dummy_univ },
+  { intros U ss, exact eq_refl },
+  { intros U ss, exact eq_symm },
+  { intros U ss, exact eq_trans },
   { intros U ss, exact function_ext },
-  { intros U ss, exact predicate_ext }
+  { intros U ss, exact relation_ext }
 end
 
 end proof
 
 namespace provable
-variables {T : preTheory L m} {T₀ : Theory L}
+open axiomatic_classical_logic' axiomatic_classical_logic
+variables {T U : preTheory L m} {T₀ : Theory L}
 
-lemma generalize {p : subformula L (m + 1) 0} (h : T.mlift ⊢ p) : T ⊢ ∀'p.pull := by rcases h; exact ⟨h.generalize⟩
+lemma generalize {p} (h : T.mlift ⊢ p) : T ⊢ ∀'p.pull := by rcases h; exact ⟨h.generalize⟩
 
-@[simp] lemma specialize {p : subformula L m 1} (t) : T ⊢ ∀'p ⟶ subst t (push p) := ⟨proof.specialize⟩
+lemma by_axiom {p} (h : p ∈ T) : T ⊢ p := ⟨proof.by_axiom h⟩
 
-@[simp] lemma univ_K (p q : subformula L m 1) : T ⊢ ∀'(p ⟶ q) ⟶ ∀'p ⟶ ∀'q := ⟨proof.univ_K⟩
+@[simp] lemma specialize {p} (t) : T ⊢ ∀'p ⟶ subst t p := ⟨proof.specialize⟩
 
-@[simp] lemma dummy_univ_quantifier (p : formula L) : T ⊢ p ⟶ ∀.(p^1) := ⟨proof.dummy_univ⟩
+@[simp] lemma dummy_univ (p q) : T ⊢ ∀'(dummy p ⟶ q) ⟶ p ⟶ ∀'q := ⟨proof.dummy_univ⟩
 
-@[simp] lemma eq_reflexivity : T₀ ⊢ ∀'(#0 =' #0) := ⟨proof.eq_reflexivity⟩
+@[simp] lemma eq_refl : T₀ ⊢ ∀'(#0 =' #0) := ⟨proof.eq_refl⟩
 
-@[simp] lemma eq_symmetry : T₀ ⊢ ∀' ∀'((#0 =' #1) ⟶ (#1 =' #0)) := ⟨proof.eq_symmetry⟩
+@[simp] lemma eq_symm : T₀ ⊢ ∀' ∀'((#0 =' #1) ⟶ (#1 =' #0)) := ⟨proof.eq_symm⟩
 
-@[simp] lemma eq_transitivity : T₀ ⊢ ∀' ∀' ∀'((#0 =' #1) ⟶ (#1 =' #2) ⟶ (#0 =' #2)) := ⟨proof.eq_transitivity⟩
+@[simp] lemma eq_trans : T₀ ⊢ ∀' ∀' ∀'((#0 =' #1) ⟶ (#1 =' #2) ⟶ (#0 =' #2)) := ⟨proof.eq_trans⟩
 
 @[simp] lemma function_ext {n} (f : L.fn n) : T₀ ⊢ eq_axiom4 f := ⟨proof.function_ext⟩
 
-@[simp] lemma predicate_ext {n} (r : L.pr n) : T₀ ⊢ eq_axiom5 r := ⟨proof.predicate_ext⟩
+@[simp] lemma relation_ext {n} (r : L.pr n) : T₀ ⊢ eq_axiom5 r := ⟨proof.relation_ext⟩
 
-
-#check @proof.rec_on
-
-@[elab_as_eliminator]
-theorem rec'_on {C : Π {m} (T : preTheory L m) (p : formula L m), T ⊢ p → Prop}
-  {T : preTheory L m} {p : formula L m} (b : T ⊢ p)
-  (mdp : ∀ {m} {T : preTheory L m} {p q : formula L m} (b₁ : T ⊢ p ⟶ q) (b₂ : T ⊢ p),
-    C T (p ⟶ q) b₁ → C T p b₂ → C T q (b₁ ⨀ b₂))
-  (by_axiom : ∀ {p : formula A} (mem : p ∈ T), C p)
-  (p0 : C ⊤)
-  (p1 : ∀ {p q : formula A}, C (p ⟶ q ⟶ p))
-  (p2 : ∀ {p q r : formula A}, C ((p ⟶ q ⟶ r) ⟶ (p ⟶ q) ⟶ p ⟶ r))
-  (p3 : ∀ {p q : formula A}, C ((∼p ⟶ ∼q) ⟶ q ⟶ p)) :
-  C p :=
+theorem rec_on {C : Π {m} (T : preTheory L m) (p : subformula L m 0), T ⊢ p → Prop}
+  {m : ℕ} {T : preTheory L m} {p : formula L m} (b : T ⊢ p)
+  (generalize : ∀ {m} {T : preTheory L m} {p} (b : T.mlift ⊢ p), C T.mlift p b → C T (∀'p.pull) (generalize b))
+  (mdp : ∀ {m} {T : preTheory L m} {p q} (b₁ : T ⊢ p ⟶ q) (b₂ : T ⊢ p), C T (p ⟶ q) b₁ → C T p b₂ → C T q (b₁ ⨀ b₂))
+  (by_axiom : ∀ {m} {T : preTheory L m} {p} (h : p ∈ T), C T p (by_axiom h))
+  (verum : ∀ {m} {T : preTheory L m}, C T ⊤ axiomatic_classical_logic'.provable_top)
+  (imply₁ : ∀ {m} {T : preTheory L m} {p q}, C T (p ⟶ q ⟶ p) (axiomatic_classical_logic'.imply₁ p q))
+  (imply₂ : ∀ {m} {T : preTheory L m} {p q r}, C T ((p ⟶ q ⟶ r) ⟶ (p ⟶ q) ⟶ p ⟶ r) (axiomatic_classical_logic'.imply₂ p q r))
+  (contra : ∀ {m} {T : preTheory L m} {p q}, C T ((∼p ⟶ ∼q) ⟶ q ⟶ p) (axiomatic_classical_logic'.contraposition p q)) 
+  (specialize : ∀ {m} {T : preTheory L m} {p} {t}, C T (∀'p ⟶ subst t p) (specialize t))
+  (dummy_univ : ∀ {m} {T : preTheory L m} {p q}, C T (∀'(dummy p ⟶ q) ⟶ p ⟶ ∀'q) (dummy_univ p q))
+  (eq_refl : ∀ {T : preTheory L 0}, C T (∀'(#0 =' #0)) eq_refl)
+  (eq_symm : ∀ {T : preTheory L 0}, C T (∀' ∀'((#0 =' #1) ⟶ (#1 =' #0))) eq_symm)
+  (eq_trans : ∀ {T : preTheory L 0}, C T (∀' ∀' ∀'((#0 =' #1) ⟶ (#1 =' #2) ⟶ (#0 =' #2))) eq_trans)
+  (function_ext : ∀ {T : preTheory L 0} {p} {f : L.fn p}, C T (eq_axiom4 f) (function_ext f))
+  (relation_ext : ∀ {T : preTheory L 0} {p} {r : L.pr p}, C T (eq_axiom5 r) (relation_ext r)) :
+  C T p b :=
 begin
   rcases b with ⟨b⟩,
   induction b,
-  case mdp : T p q bpq bp IHpq IHp { exact mdp ⟨bpq⟩ ⟨bp⟩ (IHpq @mdp @by_axiom) (IHp @mdp @by_axiom) },
-  case by_axiom : T p hp { exact by_axiom hp },
-  case verum : { exact p0 },
-  case imply₁ : { exact p1 },
-  case imply₂ : { exact p2 },
-  case contraposition { exact p3 }
+  case generalize : m T p b IH { exact generalize ⟨b⟩ IH },
+  case mdp : m T p q b₁ b₂ IH₁ IH₂ { exact mdp ⟨b₁⟩ ⟨b₂⟩ IH₁ IH₂ },
+  case by_axiom : m T p hp { exact by_axiom hp },
+  case verum : m T { exact verum },
+  case imply₁ : m T p q { exact imply₁ },
+  case imply₂ : m T p q r { exact imply₂ },
+  case contra : m T p q { exact contra },
+  case specialize : m T p t { exact specialize },
+  case dummy_univ : m T p q { exact dummy_univ },
+  case eq_refl : { exact eq_refl },
+  case eq_symm : { exact eq_symm },
+  case eq_trans : { exact eq_trans },
+  case function_ext : T p f { exact function_ext },
+  case relation_ext : T p f { exact relation_ext }
 end
 
 noncomputable def provable.proof {T : preTheory L m} {p : formula L m} (b : T ⊢ p) : T ⟹ p := nonempty.some b
 
-def deduction'_aux {q} (h : T ⟹ q) (U) (p) (hT : T = insert p U) : U ⟹ p ⟶ q :=
+def weakening_aux {p} (h : T ⊢ p) : ∀ {U}, T ⊆ U → U ⊢ p :=
 begin
-  induction h,
-  case generalize : m T q b IH
-  { have := b.generalize,
-    have : U.mlift ⟹ p.mlift ⟶ q, from IH U.mlift p.mlift (by simp[hT, preTheory.mlift_insert]),
-    have : U ⟹ (∀'(p.mlift.pull ⟶ q.pull) : subformula L _ _), from this.generalize ,
+  apply rec_on h,
+  { intros m T p b IH U hyp, refine generalize (IH $ set.image_subset _ hyp) },
+  { intros m T p q hyp_pq hyp_p IH₁ IH₂ U hyp, exact (IH₁ hyp) ⨀ (IH₂ hyp) },
+  { intros m T p hyp_p U hyp, exact by_axiom (hyp hyp_p) },
+  { intros, simp },
+  { intros, simp },
+  { intros, simp },
+  { intros, simp },
+  { intros, simp },
+  { intros, simp },
+  { intros, simp },
+  { intros, simp },
+  { intros, simp },
+  { intros, simp },
+  { intros, simp }
+end
 
-    
-     },
-  { rintros p (rfl | hp), { simp }, { exact hyp_right (by_axiom hp) q } },
+lemma deduction_aux {q} (h : T ⊢ q) : ∀ (U) (p) (hT : T = insert p U), U ⊢ p ⟶ q :=
+begin
+  apply rec_on h,
+  { rintros m T q b IH U p rfl,
+    have : U.mlift ⊢ p.mlift ⟶ q, from IH U.mlift p.mlift (by simp[preTheory.mlift_insert]),
+    have IH : U ⊢ ∀'(p.dummy ⟶ q.pull), from generalize this,
+    have : U ⊢ ∀'(p.dummy ⟶ q.pull) ⟶ p ⟶ ∀'q.pull, by simp,
+    show U ⊢ p ⟶ ∀'q.pull, from this ⨀ IH },
+  { rintros m T p₁ p₂ b₁ b₂ IH₁ IH₂ U p rfl,
+    show U ⊢ p ⟶ p₂, from (IH₁ U p rfl) ⨀₁ (IH₂ U p rfl) },
+  { rintros m T p hp U r rfl, rcases hp with (rfl | hp),
+    { simp }, { have : U ⊢ p, from by_axiom hp, exact hyp_right this r } },
+  { rintros m T U p rfl, simp },
+  { rintros m T p q U r rfl, simp },
+  { rintros m T p q r U s rfl, simp },
+  { rintros m T p q U r rfl, simp },
+  { rintros m T p t U q rfl, refine hyp_right (specialize t) _ },
+  { rintros m T p q U r rfl, refine hyp_right (dummy_univ p q) _ },
   { simp },
   { simp },
   { simp },
-  { simp }
-end
-end provable
-
-
-
-
-
-
-#check 0
-/-
-
-end proof
-
-namespace provable
-variables {T : Theory L}
-
-lemma generalize {p : formula L} (h : ⤊T ⊢ p) : T ⊢ ∀.p := by rcases h; exact ⟨h.generalize⟩
-
-@[simp] lemma specialize {p : formula L} (t) : T ⊢ ∀.p ⟶ p.rew ı[0 ⇝ t] := ⟨proof.specialize⟩
-
-@[simp] lemma univ_K (p q : formula L) : T ⊢ ∀.(p ⟶ q) ⟶ ∀.p ⟶∀.q := ⟨proof.univ_K⟩
-
-@[simp] lemma dummy_univ_quantifier (p : formula L) : T ⊢ p ⟶ ∀.(p^1) := ⟨proof.dummy_univ⟩
-
-@[simp] lemma eq_reflexivity : T ⊢ ∀.(#0 =' #0) := ⟨proof.eq_reflexivity⟩
-
-@[simp] lemma eq_symmetry : T ⊢ ∀.∀.((#0 =' #1) ⟶ (#1 =' #0)) := ⟨proof.eq_symmetry⟩
-
-@[simp] lemma eq_transitivity : T ⊢ ∀.∀.∀.((#0 =' #1) ⟶ (#1 =' #2) ⟶ (#0 =' #2)) := ⟨proof.eq_transitivity⟩
-
-@[simp] lemma function_ext {n} (f : L.fn n) : T ⊢ eq_axiom4 f := ⟨proof.function_ext⟩
-
-@[simp] lemma predicate_ext {n} (r : L.pr n) : T ⊢ eq_axiom5 r := ⟨proof.predicate_ext⟩
-
-lemma generalize_of_closed [closed_Theory T] {p} (h : T ⊢ p) : T ⊢ ∀.p :=
-by { apply generalize, simp[closed_Theory_sf_eq, h] }
-
-lemma generalize_itr : ∀ {n p}, T^n ⊢ p → T ⊢ ∀.[n] p
-| 0     p h := by simp* at*
-| (n+1) p h := by { simp at*, have := generalize_itr (generalize h), simp* at* }
-
-lemma nfal_subst : ∀ (n) (p : formula L) (s : ℕ → term L),
-  T ⊢ (∀.[n] p) ⟶ p.rew (λ x, if x < n then s x else #(x-n))
-| 0     p s := by simp
-| (n+1) p s := by { simp,
-    have lmm₁ : T ⊢ ∀.(∀.[n] p) ⟶ nfal (p.rew $ ı[0 ⇝ s n]^n) n,
-    { have := @specialize _ T (∀.[n] p) (s n), simp[formula.nfal_rew] at this,
-      exact this },
-    have s' := s,
-    have lmm₂ := nfal_subst n (p.rew $ ı[0 ⇝ s n]^n) s,
-    simp[formula.nested_rew] at lmm₂,
-    have : (λ x, (ı[0 ⇝ s n]^n $ x).rew (λ x, ite (x < n) (s x) #(x - n))) =
-      (λ x, ite (x < n + 1) (s x) #(x - (n + 1))),
-    { simp[subst_pow], ext x, have C : x < n ∨ x = n ∨ n < x, from trichotomous _ _,
-      cases C,
-      { simp[C, nat.lt.step C] }, cases C, { simp[C, term.pow_eq] },
-      { have eqn₁ : ¬x - 1 < n, from not_lt.mpr (nat.le_pred_of_lt C),
-        have eqn₂ : ¬x < n + 1, from not_lt.mpr (nat.succ_le_iff.mpr C),
-        simp[C, eqn₁, eqn₂, nat.sub_sub, add_comm 1 n] } },
-    simp[this] at lmm₂,
-    exact imply_trans lmm₁ lmm₂ }
-
-lemma nfal_subst' {n} {p : formula L} (h : T ⊢ ∀.[n] p ) (s : ℕ → term L) :
-  T ⊢ p.rew (λ x, if x < n then s x else #(x-n)) := (nfal_subst n p s) ⨀ h
-
-lemma nfal_subst'_finitary {n} {p : formula L} (h : T ⊢ ∀.[n] p ) (s : finitary (term L) n) :
-  T ⊢ p.rew (of_fin s) :=
-by { let s' : ℕ → term L := λ x, if h : x < n then s ⟨x, h⟩ else default,
-     exact cast (by { congr, ext x, by_cases C : x < n; simp[C, s'],
-       simp[show n ≤ x, from not_lt.mp C] }) (nfal_subst' h s')}
-
-lemma fal_complete_rew (p : formula L) (s : ℕ → term L) :
-  T ⊢ (∀.* p) ⟶ p.rew s :=
-begin
-  have : T ⊢ (∀.* p) ⟶ p.rew (λ x, if x < p.arity then s x else #(x - p.arity)),
-    from nfal_subst p.arity p s,
-  have eqn : (p.rew (λ x, if x < p.arity then s x else #(x - p.arity))) = p.rew s,
-    from formula.rew_rew p (λ m h, by simp[h]),
-  simp[eqn] at this, exact this
+  { rintros T _ f U p rfl, refine hyp_right (function_ext f) _ },
+  { rintros T _ f U p rfl, refine hyp_right (relation_ext f) _ }
 end
 
-lemma weakening {p} (h : T ⊢ p) {U} (ss : T ⊆ U) : U ⊢ p :=
-by rcases h; exact ⟨h.weakening ss⟩
+instance : axiomatic_classical_logic (formula L m) :=
+{ deduction' := λ T p q h, deduction_aux h T p rfl,
+  weakening := λ T U p ss b, weakening_aux b ss }
 
-lemma weakening' {U : Theory L} {p : formula L} : T ⊆ U → T ⊢ p → U ⊢ p := λ hi hp,
-weakening hp hi
+lemma empty_axiom_generalize {p : formula L (m + 1)} (hp : ⬝⊢ p) : ⬝⊢ ∀'p.pull :=
+by { have : preTheory.mlift ∅ ⊢ p, by simpa[preTheory.mlift] using hp, exact generalize this }
 
-private lemma delete_imply {p} (h : T ⊢ p) : ∀ q, T \ {q} ⊢ q ⟶ p :=
+private lemma mlift_list_conjunction (P₀ : list (formula L $ m + 1)) : (∀ p, p ∈ P₀ → p ∈ T.mlift) →
+  ∃ P : list (formula L m), P.conjunction.mlift = P₀.conjunction ∧ (∀ p, p ∈ P → p ∈ T) :=
 begin
-  rcases h,
-  induction h with T p hyp_p IH T p₁ p₂ hyp_p₁₂ hyp_p₁ IH₁ IH₂ T p hyp_p;
-    try { intros q, simp }; intros q,
-  { have IH : ⤊T \ {q^1} ⊢ q^1 ⟶ p := IH (q^1),
-    have lmm₁ : T \ {q} ⊢ q ⟶ ∀.(q^1), { simp },
-    have lmm₂ : T \ {q} ⊢ ∀.(q^1) ⟶ ∀.p,
-    { suffices : T \ {q} ⊢ ∀.(q^1 ⟶ p),
-      { have lmm : T \ {q} ⊢ ∀.(q^1 ⟶ p) ⟶ ∀.(q^1) ⟶ ∀.p, simp,
-        exact lmm ⨀ this },
-      refine generalize (weakening IH (λ x h, _)), 
-      rcases h with ⟨h, neq⟩, rcases h with ⟨p', h', rfl⟩,
-      refine ⟨p', ⟨h', λ c, _⟩, rfl⟩, simp at c,
-      rw c at neq, exact neq rfl },
-    exact imply_trans lmm₁ lmm₂ },
-  { have : T \ {q} ⊢ (q ⟶ p₁ ⟶ p₂) ⟶ (q ⟶ p₁) ⟶ (q ⟶ p₂), simp, 
-    have : T \ {q} ⊢ (q ⟶ p₁) ⟶ q ⟶ p₂, from this ⨀ (IH₁ _),
-    exact this ⨀ (IH₂ _) },
-  { by_cases eqn : p = q,
-    { simp[eqn] },
-    { have : T \ {q} ⊢ p, from by_axiom ⟨hyp_p, eqn⟩,
-      simp[this] } }
+  induction P₀ with p₀ P₀ IH,
+  { intros _, refine ⟨[], by simp⟩ },
+  { intros h,
+    have : ∃ P : list (formula L m), P.conjunction.mlift = P₀.conjunction ∧ (∀ p, p ∈ P → p ∈ T),
+    from IH (λ p hp, h p (by simp[hp])),
+    rcases this with ⟨P, eq, hP⟩,
+    have : p₀ ∈ T.mlift, from h p₀ (by simp), rcases this with ⟨p, hp, rfl⟩,
+    refine ⟨p :: P, by simpa using eq, by { rintros q (rfl | hq), { exact hp }, { exact hP q hq } }⟩ }
 end
 
-instance : axiomatic_classical_logic (formula L) :=
-{ deduction' := λ T p q h, by { have : (T+{p}) \ {p} ⊢ p ⟶ q, from delete_imply h p,
-    refine weakening this (λ x h, _), rcases h with ⟨h, neq⟩,
-    cases h; simp* at* },
-  weakening := @weakening' L }
-
-@[elab_as_eliminator]
-theorem rec'_on {T : Theory L} {C : ℕ → formula L → Prop} {i : ℕ} {p : formula L} (b : T^i ⊢ p)
-  (GE : ∀ {i} {p : formula L} (b : T^(i + 1) ⊢ p), C (i + 1) p → C i (∀.p))
-  (MP : ∀ {i} {p q : formula L} (b₁ : T^i ⊢ p ⟶ q) (b₂ : T^i ⊢ p), C i (p ⟶ q) → C i p → C i q)
-  (by_axiom : ∀ {i} {p : formula L} (mem : p ∈ T^i), C i p)
-  (p0 : ∀ {i}, C i ⊤)
-  (p1 : ∀ {i} {p q : formula L}, C i (p ⟶ q ⟶ p))
-  (p2 : ∀ {i} {p q r : formula L}, C i ((p ⟶ q ⟶ r) ⟶ (p ⟶ q) ⟶ p ⟶ r))
-  (p3 : ∀ {i} {p q : formula L}, C i ((∼p ⟶ ∼q) ⟶ q ⟶ p))
-  (q1 : ∀ {i} {p : formula L} {t : term L}, C i (∀.p ⟶ p.rew ı[0 ⇝ t]))
-  (q2 : ∀ {i} {p q : formula L}, C i (∀.(p ⟶ q) ⟶ ∀.p ⟶∀.q))
-  (q3 : ∀ {i} {p : formula L}, C i (p ⟶ ∀.(p^1)))
-  (e1 : ∀ {i}, C i (∀.(#0 =' #0)))
-  (e2 : ∀ {i}, C i (∀.∀.((#0 =' #1) ⟶ (#1 =' #0))))
-  (e3 : ∀ {i}, C i (∀.∀.∀.((#0 =' #1) ⟶ (#1 =' #2) ⟶ (#0 =' #2))))
-  (e4 : ∀ {i} {m} {f : L.fn m}, C i (eq_axiom4 f))
-  (e5 : ∀ {i} {m} {r : L.pr m}, C i (eq_axiom5 r)) :
- C i p :=
+theorem finite_character_aux {m} {T : preTheory L m} {p} :
+  T ⊢ p → ∃ P : list (formula L m), (∀ p, p ∈ P → p ∈ T) ∧ ⬝⊢ P.conjunction ⟶ p := λ h,
 begin
-  suffices :
-    ∀ {p : formula L} {U : Theory L} (b : U ⊢ p) {i : ℕ} (ss : U ⊆ T^i),  C i p,
-  { refine this b (by refl) },
-  rintros p U ⟨b⟩,
-  induction b,
-  case generalize : U p b IH
-  { intros i ss,
-    have ss' : ⤊U ⊆ T ^ (i + 1), { rintros _ ⟨q, mem, rfl⟩, simp[Theory.sf_itr_succ], refine ⟨q, ss mem, rfl⟩ },
-    have : C (i + 1) p, from @IH (i + 1) ss',
-    refine GE (weakening ⟨b⟩ ss') this },
-  case mdp : U p q b₁ b₂ IH₁ IH₂
-  { intros i ss, refine MP (weakening ⟨b₁⟩ ss) (weakening ⟨b₂⟩ ss) (IH₁ ss) (IH₂ ss) },
-  case by_axiom : U p mem
-  { intros i ss, refine by_axiom (ss mem) },
-  { refine λ i ss, p0 },
-  { refine λ i ss, p1 },
-  { refine λ i ss, p2 },
-  { refine λ i ss, p3 },
-  { refine λ i ss, q1 },
-  { refine λ i ss, q2 },
-  { refine λ i ss, q3 },
-  { refine λ i ss, e1 },
-  { refine λ i ss, e2 },
-  { refine λ i ss, e3 },
-  { refine λ i ss, e4 },
-  { refine λ i ss, e5 }
-end
-
-theorem proof_compact : ∀ {T : ℕ → Theory L}, (∀ s, T s ⊆ T (s+1)) →
-  ∀ {p}, (⋃ s, T s) ⊢ p → ∃ s, T s ⊢ p :=
-begin
-  suffices : ∀ {p} {U : Theory L}, U ⊢ p → ∀ {T : ℕ → Theory L},
-    (∀ s, T s ⊆ T (s+1)) → U ⊆ (⋃ s, T s) → ∃ s, T s ⊢ p,
-  { refine λ T hyp p h, this h hyp (λ x hx, hx) },
-  rintros p U ⟨b⟩,
-  induction b,
-  case generalize : T p h IH
-  { intros U hyp ss,
-    let U' := λ s, ⤊(U s),
-    have hyp' : ∀ s, U' s ⊆ U' (s + 1),
-    { simp[U'], intros s p hyp_p, exact hyp s hyp_p },
-    have ss' : ⤊T ⊆ ⋃ s, U' s,
-    { intros q hyp_q, rcases hyp_q with ⟨q', hyp_q', rfl⟩, rcases (ss hyp_q') with ⟨_, ⟨s, rfl⟩, hyp_s⟩,
-      simp, refine ⟨s, _, hyp_s, rfl⟩ },
-    have : ∃ s, U' s ⊢ p, from IH hyp' ss', rcases this with ⟨s, h⟩,
-    refine ⟨s, generalize h⟩ },
-  case mdp : T p q hyp_pq hyp_p IH₁ IH₂
-  { intros U hyp ss,
-    have : ∃ s, U s ⊢ p ⟶ q, from IH₁ hyp ss, rcases this with ⟨s₁, lmm₁⟩,
-    have : ∃ s, U s ⊢ p, from IH₂ hyp ss, rcases this with ⟨s₂, lmm₂⟩,
-    refine ⟨max s₁ s₂, _⟩,
-    have lmm₁ : U (max s₁ s₂) ⊢ p ⟶ q, from provable.weakening lmm₁ (ss_le hyp (by simp)),
-    have lmm₂ : U (max s₁ s₂) ⊢ p, from provable.weakening lmm₂ (ss_le hyp (by simp)),
-    exact lmm₁ ⨀ lmm₂ },
-  case by_axiom : T p hyp_p
-  { intros U hyp ss, rcases (ss hyp_p) with ⟨_, ⟨s, rfl⟩, hyp_s⟩,
-    refine ⟨s, by_axiom hyp_s⟩ },
-  { refine λ _ _ _, ⟨0, by simp⟩ },
-  { refine λ _ _ _, ⟨0, by simp⟩ },
-  { refine λ _ _ _, ⟨0, by simp⟩ },
-  { refine λ _ _ _, ⟨0, by simp⟩ },
-  { refine λ _ _ _, ⟨0, by simp⟩ },
-  { refine λ _ _ _, ⟨0, by simp⟩ },
-  { refine λ _ _ _, ⟨0, by simp⟩ },
-  { refine λ _ _ _, ⟨0, by simp⟩ },
-  { refine λ _ _ _, ⟨0, by simp⟩ },
-  { refine λ _ _ _, ⟨0, by simp⟩ },
-  { refine λ _ _ _, ⟨0, by simp⟩ },
-  { refine λ _ _ _, ⟨0, by simp⟩ }
-end
-
-lemma inf_conjunction_mem {n : ℕ} {P : finitary (formula L) n} :
-  ∀ {p}, p ∈ P → T ⊢ inf_conjunction n P ⟶ p :=
-begin
-  induction n with n IH; simp[inf_conjunction];
-  simp[has_mem.mem, finitary.mem],
-  intros p mem,
-  exact and_imply_of_imply_right (IH mem)
-end
-
-private lemma list_conjunction_sf (P₀ : list (formula L)) : (∀ p, p ∈ P₀ → ⤊T p) →
-  ∃ P : list (formula L), (P.conjunction)^1 = P₀.conjunction ∧ (∀ p, p ∈ P → T p) :=
-begin
-  induction P₀ with p₀ P₀ IHl, { refine λ _, ⟨[], _⟩, simp },
-  { intros hyp,
-    have : ∀ p, p ∈ P₀ → ⤊T p,
-    { intros p hyp_p, refine hyp _ _, simp[hyp_p] },
-    rcases IHl this with ⟨P, hyp_P⟩,
-    have := hyp p₀ (by simp),
-    rcases this with ⟨p, hyp_p, rfl⟩,
-    have lmm₁ : ((p :: P).conjunction)^1= (p^1 :: P₀).conjunction,
-    { simp[hyp_P] },
-    have lmm₂ : ∀ (q : formula L), q ∈ (p :: P) → T q,
-    { simp, refine ⟨hyp_p, hyp_P.2⟩ },
-    refine ⟨p :: P, lmm₁, lmm₂⟩ }
-end
-
-private lemma list_conjunction_rew_eq : ∀ (P : list (formula L)) (s),
-  P.conjunction.rew s = list.conjunction (P.map (λ p, p.rew s))
-| []       _ := by simp[formula.rew]
-| (p :: P) s := by simp[formula.rew, list_conjunction_rew_eq P]
-
-theorem proof_conjunction {T : Theory L} {p} :
-  T ⊢ p → ∃ P : list (formula L), (∀ p, p ∈ P → T p) ∧ ∅ ⊢ P.conjunction ⟶ p := λ h,
-begin
-  rcases h,
-  induction h,
-  case generalize : T p hyp IH
-  { rcases IH with ⟨P₀, hyp_P₀, prov⟩,
-    have : ∃ P : list (formula L), (P.conjunction)^1 = P₀.conjunction ∧ ∀ p, p ∈ P → T p,
-    from list_conjunction_sf _ hyp_P₀,
-    rcases this with ⟨P, eqn, hyp_P⟩,
-    have : ∅ ⊢ P.conjunction ⟶ ∀.p,
-    { refine deduction.mp (generalize _),
-      rw [←sf_dsb, eqn], refine deduction.mpr (weakening prov (λ x hx, _)), cases hx },
-    refine ⟨P, hyp_P, this⟩ },
-  case mdp : T p q hyp_pq hyp_p IH₁ IH₂
-  { rcases IH₁ with ⟨P₁, IH₁, prov₁⟩, rcases IH₂ with ⟨P₂, IH₂, prov₂⟩,
+  apply rec_on h,
+  { rintros m T p b ⟨P₀, IH, IHb⟩,
+    have : ∃ P : list (formula L m), P.conjunction.mlift = P₀.conjunction ∧ ∀ p, p ∈ P → p ∈ T,
+    from mlift_list_conjunction P₀ IH,
+    rcases this with ⟨P, eqP, hP⟩,
+    refine ⟨P, hP, _⟩,
+    have : ⬝⊢ ∀'(P.conjunction.dummy ⟶ p.pull),
+    { have := empty_axiom_generalize IHb, rw[←eqP] at this; exact this },
+    exact dummy_univ P.conjunction p.pull ⨀ this },
+  { rintros m T p q b₁ b₂ ⟨P₁, IH₁, IHb₁⟩ ⟨P₂, IH₂, IHb₂⟩,
     refine ⟨P₁ ++ P₂, _, _⟩,
-    { simp, intros p h, cases h, refine IH₁ _ h, refine IH₂ _ h },
-    { have : ∅+{(P₁ ++ P₂).conjunction} ⊢ P₂.conjunction, from deduction.mpr (list_conjunction_weakening (by simp)),
-      have lmm₁ : ∅+{(P₁ ++ P₂).conjunction} ⊢ p,
-        from (show _ ⊢ P₂.conjunction ⟶ p, from weakening_insert prov₂ _) ⨀ this,
-      have : ∅+{(P₁ ++ P₂).conjunction} ⊢ P₁.conjunction, from deduction.mpr (list_conjunction_weakening (by simp)),
-      have lmm₂ : ∅+{(P₁ ++ P₂).conjunction} ⊢ p ⟶ q,
-      from (show _ ⊢ P₁.conjunction ⟶ p ⟶ q, from weakening_insert prov₁ _) ⨀ this,
-      refine deduction.mp (lmm₂ ⨀ lmm₁) } },
-  case by_axiom : T p hyp_p
-  { refine ⟨[p], _⟩, simp,
-    have : ∅ ⊢ p ⊓ ⊤ ⟶ p,
-    { apply deduction.mp,
-      have : ∅+{p ⊓ ⊤} ⊢ p ⊓ ⊤, from insert (p ⊓ ⊤),
-      simp[*, axiomatic_classical_logic'.iff_and] at* },
-    refine hyp_p },
-  { refine ⟨[], _⟩, simp },
-  { refine ⟨[], _⟩, simp },
-  { refine ⟨[], _⟩, simp },
-  { refine ⟨[], _⟩, simp },
-  { refine ⟨[], _⟩, simp },
-  { refine ⟨[], _⟩, simp },
-  { refine ⟨[], _⟩, simp },
-  { refine ⟨[], _⟩, simp },
-  { refine ⟨[], _⟩, simp },
-  { refine ⟨[], _⟩, simp },
-  { refine ⟨[], _⟩, simp },
-  { refine ⟨[], _⟩, simp }
+    { simp, rintros p (hp | hp), { exact IH₁ p hp }, { exact IH₂ p hp } },
+    { have    : ⬝⊢ (P₁ ++ P₂).conjunction ⟶ P₁.conjunction, from list_conjunction_weakening (by simp),
+      have h₁ : ⬝⊢ (P₁ ++ P₂).conjunction ⟶ p ⟶ q, from imply_trans this IHb₁,
+      have    : ⬝⊢ (P₁ ++ P₂).conjunction ⟶ P₂.conjunction, from list_conjunction_weakening (by simp),
+      have h₂ : ⬝⊢ (P₁ ++ P₂).conjunction ⟶ p, from imply_trans this IHb₂,
+      exact h₁ ⨀₁ h₂ } },
+  { rintros m T p hp, refine ⟨[p], by simp[hp], _⟩, simp, refine deduction.mp (by simp) },
+  { rintros m T, refine ⟨[], by simp, by simp[empty_axiom]⟩ },
+  { rintros m T p q, refine ⟨[], by simp, by simp[empty_axiom]⟩ },
+  { rintros m T p q r, refine ⟨[], by simp, by simp[empty_axiom]⟩ },
+  { rintros m T p q, refine ⟨[], by simp, by simp[empty_axiom]⟩ },
+  { rintros m T p t, refine ⟨[], by simp, by simp[empty_axiom]⟩ },
+  { rintros m T p q, refine ⟨[], by simp, by simp[empty_axiom]⟩ },
+  { rintros T, refine ⟨[], by simp, by simp[empty_axiom]⟩ },
+  { rintros T, refine ⟨[], by simp, by simp[empty_axiom]⟩ },
+  { rintros T, refine ⟨[], by simp, by simp[empty_axiom]⟩ },
+  { rintros T p f, refine ⟨[], by simp, by simp[empty_axiom]⟩ },
+  { rintros T p r, refine ⟨[], by simp, by simp[empty_axiom]⟩ },
 end
 
-instance : Theory.has_finite_character (formula L) :=
-Theory.finite_character_of_finite_probable (formula L) (λ T p, proof_conjunction)
-
-theorem proof_conjunction_union {T U : Theory L} {p} :
-  T ∪ U ⊢ p → ∃ P Q : list (formula L), (∀ p, p ∈ P → T p) ∧ (∀ p, p ∈ Q → U p) ∧
-  ∅ ⊢ P.conjunction ⟶ Q.conjunction ⟶ p := λ h,
-begin
-  rcases proof_conjunction h with ⟨R, hR, b⟩,
-  let P := R.filter (λ p, p ∈ T),
-  let Q := R.filter (λ p, p ∈ U),
-  refine ⟨P, Q, by { simp, intros p _ h, exact h }, by { simp, intros p _ h, exact h }, _⟩,
-  refine (deduction.mp $ deduction.mp _),
-  have : ∅ +{ P.conjunction } +{ Q.conjunction } ⊢ R.conjunction,
-  refine list_conjunction_provable _,
-  { intros p memR, rcases hR p memR with (memT | memU),
-    { have : p ∈ P, by simp[memR, memT], refine list_conjunction_mem this ⨀ (by simp[-insert_emptyc_eq]) },
-    { have : p ∈ Q, by simp[memR, memU], refine list_conjunction_mem this ⨀ (by simp[-insert_emptyc_eq]) } },
-  exact (weakening b (by simp)) ⨀ this
-end
-
-lemma fal_subst {p} (h : T ⊢ ∀.p) (t) : T ⊢ p.rew ı[0 ⇝ t] :=
-(show T ⊢ ∀.p ⟶ p.rew ı[0 ⇝ t], by simp) ⨀ h
-
-infixl ` ⊚ `:60 := fal_subst
-
-lemma add_sf (p) : ⤊(T +{ ∀.p }) ⊢ p :=
-by { have : ⤊(T +{∀.p}) ⊢ (∀.p)^1, rw ← sf_dsb, simp, 
-     have := fal_subst this #0, simp[formula.nested_rew] at this,
-     exact this }
-
-lemma cl_prove_rew [cl : closed_Theory T] : ∀ {p : formula L}, T ⊢ p → ∀ s, T ⊢ p.rew s :=
-begin
-  suffices : ∀ {p : formula L} {T}, T ⊢ p → closed_Theory T → ∀ s, T ⊢ p.rew s,
-  { refine λ p h s, this h cl _ },
-  rintros p T ⟨b⟩,
-  induction b,
-  case generalize : T p hyp IH
-  { intros cl s, rw[@closed_Theory_sf_eq _ _ cl] at IH,
-    refine generalize _, simp[@closed_Theory_sf_eq _ _ cl], exact IH cl _ },
-  case mdp : T p q hyp_pq hyp_p IH₁ IH₂
-  { intros cl s, simp[formula.rew, @closed_Theory_sf_eq _ _ cl] at*, refine (IH₁ cl _) ⨀ (IH₂ cl _) },
-  case by_axiom : T p hyp
-  { intros cl s, simp[show is_sentence p, by exactI closed_Theory.cl hyp], exact by_axiom hyp },
-  { simp },
-  { simp },
-  { simp },
-  { simp },
-  { intros, simp[formula.rew, formula.subst_sf_rew] },
-  { simp },
-  case dummy_univ : T p { intros,
-    simp,
-    have : (p^1).rew (s^1) = (p.rew s)^1,
-    { simp[formula.pow_eq, formula.rew, formula.nested_rew], refl },
-    simp[this] },
-  { simp },
-  { simp },
-  { simp },
-  { simp [formula.is_sentence_rew eq_axiom4_is_sentence] },
-  { simp [formula.is_sentence_rew eq_axiom5_is_sentence] }
-end
-
-lemma pow_of_cl [closed_Theory T] {p : formula L} (i : ℕ) : T ⊢ p → T^i ⊢ p :=
-by simp[closed_Theory_pow_eq]
-
-lemma iff_fal_complete [closed_Theory T] {p : formula L} : T ⊢ p ↔ T ⊢ ∀.* p :=
-⟨λ h, generalize_itr (pow_of_cl p.arity h), λ h, by simpa using fal_complete_rew p ı ⨀ h⟩
-
-lemma pp_prove_rew {n} (pp : proper_at n T) :
-  ∀ {p : formula L}, T ⊢ p → ∀ s, T ⊢ p.rew (s^n) :=
-begin
-  suffices : ∀ {p : formula L} {T},
-    T ⊢ p → ∀ {n}, proper_at n T → ∀ s, T ⊢ p.rew (s^n),
-  { refine λ p h s, this h @pp _ },
-  rintros p T ⟨b⟩,
-  induction b,
-  case generalize : T p hyp IH
-  { intros n pp s,
-    refine generalize _, refine @IH (n+1) (@proper_Theory_sf_itr _ _ _ @pp 1) s },
-  case mdp : T p q hyp_pq hyp_p IH₁ IH₂
-  { intros n pp s, refine (IH₁ @pp _) ⨀ (IH₂ @pp _) },
-  case by_axiom : T p hyp
-  { intros n pp s, refine by_axiom (pp _ _ hyp) },
-  { simp },
-  { simp },
-  { simp },
-  { simp },
-  { intros, simp[formula.subst_sf_rew] },
-  { simp },
-  case dummy_univ : T p { intros,
-    simp,
-    simp[←formula.pow_rew_distrib] },
-  { simp },
-  { simp },
-  { simp },
-  { simp [formula.is_sentence_rew eq_axiom4_is_sentence] },
-  { simp [formula.is_sentence_rew eq_axiom5_is_sentence] },
-end
-
-lemma proper_Theory_pow_rew (n : ℕ) [proper_Theory T] : ∀ {p : formula L},
-  T^n ⊢ p → ∀ s, T^n ⊢ p.rew (s^n) := @pp_prove_rew L (T^n) n (properc_Theory_sf_itr)
-
-lemma proper_Theory_rew [proper_Theory T] : ∀ {p : formula L},
-  T ⊢ p → ∀ s, T ⊢ p.rew s := @pp_prove_rew _ _ 0 proper_Theory.proper
-
-protected lemma sup_disjunction {n} {P : finitary (formula L) n} (i) (h : T ⊢ P i) : T ⊢ sup_disjunction n P :=
-by { induction n with n IH; simp, { exfalso, exact i.val.not_lt_zero i.property },
-     { rcases i with ⟨i, hi⟩,
-       have : i = n ∨ i < n, exact eq_or_lt_of_le (nat.lt_succ_iff.mp hi), rcases this with (rfl | lt),
-       { refine imply_or_left _ _ ⨀ h }, { simpa using imply_or_right _ _ ⨀ (@IH (λ i, P i) ⟨i, lt⟩ (by simp; exact h)) } } }
-
-lemma sf_sf {p : formula L} : ⤊T ⊢ p^1 ↔ T ⊢ p :=
-⟨λ h, by { have := fal_subst (generalize h) #0, simp* at* },
- λ h, by { have : ∃ P : list (formula L), (∀ p, p ∈ P → p ∈ T) ∧ ∅ ⊢ P.conjunction ⟶ p,
-  from proof_conjunction h, rcases this with ⟨P, hyp_P, prov⟩,
-  have lmm₁ : ⤊T ⊢ list.conjunction (P.map (λ p, p^1)),
-  { refine list_conjunction_provable (λ p hyp, by_axiom _), simp at hyp, rcases hyp with ⟨p', p'_mem, rfl⟩,
-    refine ⟨p', hyp_P p' p'_mem, rfl⟩ },
-  have lmm₂ : ⤊T ⊢ list.conjunction (P.map (λ p, p^1)) ⟶ p^1,
-  { have : ∅ ⊢ (P.conjunction)^1 ⟶ p^1, by exactI cl_prove_rew prov _,
-    simp[formula.pow_eq, list_conjunction_rew_eq] at this,
-    refine weakening this (λ p h, _), exfalso, exact h },
-  refine lmm₂ ⨀ lmm₁ }⟩
-
-lemma sf_itr_sf_itr : ∀ {i : ℕ} {p : formula L},
-  T^i ⊢ p^i ↔ T ⊢ p
-| 0     p := by simp
-| (i+1) p := by simp[Theory.sf_itr_succ];
-    rw [show p^(i + 1) = (p^i)^1, by simp[formula.pow_add], sf_sf, @sf_itr_sf_itr i]
-
-lemma pow_rew' [proper_Theory T] (i : ℕ) {p : formula L} (h : T^(i + 1) ⊢ p) (s u : ℕ → term L) :
-  T^i ⊢ p.rew (λ x, if x < i + 1 then s x else (u (x - i - 1))^i) :=
-begin
-  have t := #0,
-  let f : ℕ → term L := λ x, if x < i + 1 then s x else (u (x - i - 1))^i,
-  have : T^i ⊢ ∀.(∀.[i + 1] p) ^ (i+1),
-    from generalize (show T^(i + 1) ⊢ (∀.[i + 1] p) ^ (i+1), from sf_itr_sf_itr.mpr (generalize_itr h)),
-  have := fal_subst this t,
-  have := (proper_Theory_pow_rew i this u),
-  simp[formula.nfal_pow, formula.nested_rew, -nfal] at this,
-  have := nfal_subst' this s, simp[formula.nested_rew, term.nested_rew, ı] at this,
-  simp[subst_pow, rewriting_sf_itr.pow_add] at this,
-  have eqn : (λ x, (ite (x < i + 1) #x #(x + (i + 1))).rew (λ x, (ı[(i + 1) ⇝ t ^ (i + 1)] x).rew
-    (λ x, (u^(i + (i + 1)) $ x).rew (λ x, ite (x < i+1) (s x) #(x - (i+1))) ))) = f,
-  { funext x₀, by_cases C : x₀ < i + 1; simp[C],
-    { simp[f, rewriting_sf_itr.pow_eq'],
-      have : x₀ < i + (i + 1), exact nat.lt_add_left _ _ _ C,
-      simp[this, C] },
-    { have : i + 1 < x₀ + (i + 1), { omega },
-      simp[f, this, rewriting_sf_itr.pow_eq', term.pow_eq], 
-      have : ¬x₀ + i < i + (i + 1), { omega }, simp[this],
-      have e₁ : ∀ x, ¬x + (i + (i + 1)) < i + 1, { intros x, omega },
-      have e₂ : ∀ x, x + (i + (i + 1)) - (i + 1) = x + i, { omega },
-      simp[e₁, e₂],
-      have : i + 1 ≤ x₀, { exact not_lt.mp C },
-      simp[←nat.sub_sub, C] } },
-  rw eqn at this,
-  exact this
-end
-
-lemma pow_subst' [proper_Theory T] (i : ℕ) {p : formula L} (h : T^(i + 1) ⊢ p) (t : term L) :
-  T^i ⊢ p.rew ı[i ⇝ t] :=
-by { have := pow_rew' i h ı[i ⇝ t] ı,
-     have eqn : (λ x, ite (x < i + 1) (ı[i ⇝ t] x) (ı (x - i - 1) ^ i)) = ı[i ⇝ t],
-     { funext x, by_cases C₁ : x < i + 1; simp[C₁],
-       have : i < x, exact nat.succ_le_iff.mp (not_lt.mp C₁),
-       simp[this, ı], omega },
-     rw eqn at this, exact this }
-
-lemma use {p : formula L} (t) (h : T ⊢ p.rew ı[0 ⇝ t]) : T ⊢ ∃.p :=
-begin
-  simp[has_exists_quantifier.ex, formula.ex],
-  refine raa (p.rew ı[0 ⇝ t]) (by simp[h]) (deduction.mpr _),
-  have : ∼p.rew ı[0 ⇝ t] = (∼p).rew ı[0 ⇝ t] := rfl,
-  rw[this], refine specialize t,
-end
-
-lemma use_0 {p : formula L} (h : ⤊T ⊢ p) : T ⊢ ∃.p :=
-use #0 ((generalize h) ⊚ #0)
-
-@[simp] lemma eq_refl : ∀ {t : term L}, T ⊢ t =' t := (@eq_reflexivity _ T).fal_subst
-
-lemma eq_symm : ∀ {t u : term L}, (T ⊢ t =' u) → (T ⊢ u =' t) :=
-begin
-  intros t u h,
-  have : T ⊢ (t =' u) ⟶ (u =' t), { have := fal_subst (fal_subst (@eq_symmetry _ T) u) t, simp at*, refine this },
-  refine this ⨀ h
-end
-
-lemma eq_trans {t₁ t₂ t₃ : term L} : (T ⊢ t₁ =' t₂) → (T ⊢ t₂ =' t₃) → (T ⊢ t₁ =' t₃) := λ h₁ h₂,
-by { have : T ⊢ (t₁ =' t₂) ⟶ (t₂ =' t₃) ⟶ (t₁ =' t₃),
-     { have := (@eq_transitivity _ T) ⊚ t₃ ⊚ t₂ ⊚ t₁, simp[←term.pow_rew_distrib] at*,
-       exact this },
-     exact (this ⨀ h₁) ⨀ h₂ }
-
-lemma ne_symm {t u : term L} (h : T ⊢ t ≄ u) : T ⊢ u ≄ t :=
-neg_of_equiv h (show T ⊢ (t =' u) ⟷ (u =' t), by { 
-    have : T ⊢ (t =' u) ⟶ (u =' t),
-    { have := fal_subst (fal_subst (@eq_symmetry _ T) u) t, simp at*, refine this },
-    have : T ⊢ (u =' t) ⟶ (t =' u),
-    { have := fal_subst (fal_subst (@eq_symmetry _ T) t) u, simp at*, refine this },
-    simp[iff_equiv, *] })
-
-lemma function_ext' {n} (f : L.fn n) (v₁ v₂ : finitary (term L) n) :
-  T ⊢ (⋀ i, v₁ i =' v₂ i) ⟶ (term.app f v₁ =' term.app f v₂) :=
-begin
-  let s : ℕ → term L :=
-    (λ x, if h₁ : x < n then v₁ ⟨x, h₁⟩ else
-          if h₂ : x < 2*n then v₂ ⟨x - n, by { simp[two_mul] at*, omega}⟩ else #x),
-  have eq_conj :
-    (λ i, ite (↑i < 2 * n) (s ↑i) #(↑i - 2*n) =' ite (n + ↑i < 2*n) (s (n + ↑i)) #(n + ↑i - 2*n) : fin n → formula L) =
-    (λ i, v₁ i =' v₂ i),
-  { funext i, simp[s, two_mul, show ↑i < n, from i.property],
-    intros h, exfalso, refine not_le_of_gt i.property (le_of_add_le_left h) },      
-  have eq_v₁ : (λ i, ite (↑i < 2 * n) (s ↑i) #(↑i - 2 * n)) = v₁,
-  { funext i, simp[s, two_mul, show ↑i < n, from i.property],
-    intros h, exfalso, refine not_le_of_gt i.property (le_of_add_le_left h) },
-  have eq_v₂ : (λ i, ite (n + ↑i < 2 * n) (s (n + ↑i)) #(n + ↑i - 2 * n)) = v₂,
-  { funext i, simp[s, two_mul, show ↑i < n, from i.property] },
-  have := nfal_subst' (@function_ext _ T _ f) s,
-  simp[eq_conj, eq_v₁, eq_v₂] at this, exact this
-end
-
-lemma predicate_ext' {n} (r : L.pr n) (v₁ v₂ : finitary (term L) n) :
-  T ⊢ (⋀ i, v₁ i =' v₂ i) ⟶ formula.app r v₁ ⟶ formula.app r v₂ :=
-begin
-  let s : ℕ → term L :=
-    (λ x, if h₁ : x < n then v₁ ⟨x, h₁⟩ else
-          if h₂ : x < 2*n then v₂ ⟨x - n, by { simp[two_mul] at*, omega}⟩ else #x),
-  have eq_conj :
-    (λ i, ite (↑i < 2 * n) (s ↑i) #(↑i - 2*n) =' ite (n + ↑i < 2*n) (s (n + ↑i)) #(n + ↑i - 2*n) : fin n → formula L) =
-    (λ i, v₁ i =' v₂ i),
-  { funext i, simp[s, two_mul, show ↑i < n, from i.property],
-    intros h, exfalso, refine not_le_of_gt i.property (le_of_add_le_left h) },      
-  have eq_v₁ : (λ i, ite (↑i < 2 * n) (s ↑i) #(↑i - 2 * n)) = v₁,
-  { funext i, simp[s, two_mul, show ↑i < n, from i.property],
-    intros h, exfalso, refine not_le_of_gt i.property (le_of_add_le_left h) },
-  have eq_v₂ : (λ i, ite (n + ↑i < 2 * n) (s (n + ↑i)) #(n + ↑i - 2 * n)) = v₂,
-  { funext i, simp[s, two_mul, show ↑i < n, from i.property] },
-  have := nfal_subst' (@predicate_ext _ T _ r) s,
-  simp[eq_conj, eq_v₁, eq_v₂] at this, exact this
-end
-
-lemma predicate_ext'' {n} (r : L.pr n) (v₁ v₂ : finitary (term L) n) :
-  T ⊢ (⋀ i, v₁ i =' v₂ i) ⟶ (formula.app r v₁ ⟷ formula.app r v₂) :=
-by { refine deduction.mp _,
-     simp[iff_equiv], split,
-     { refine (predicate_ext' r v₁ v₂) ⨀ (by simp) },
-     { refine (predicate_ext' r v₂ v₁) ⨀
-       (conjunction_iff.mpr (λ i, eq_symm (deduction.mpr $ inf_conjunction_mem $ finitary.index_mem _ i))) } }
-
-lemma equal_rew_equal (s₁ s₂ : ℕ → term L) (e : ∀ n, T ⊢ s₁ n =' s₂ n) : ∀ (t : term L) ,
-  T ⊢ t.rew s₁ =' t.rew s₂
-| (#n)                := by simp; exact e _
-| (@term.app _ n f v) :=
-  by { simp,
-       have : T ⊢ inf_conjunction n (λ i, (v i).rew s₁ =' (v i).rew s₂),
-       { simp, intros i, refine equal_rew_equal (v i) },
-       refine (@function_ext' _ T _ f (λ i, (v i).rew s₁) (λ i, (v i).rew s₂)) ⨀ this }
-
-lemma equal_fal_subst_equal (t : term L) {t₁ t₂} (h : T ⊢ t₁ =' t₂) :
-  T ⊢ t.rew (t₁ ⌢ ı) =' t.rew (t₂ ⌢ ı) :=
-by { refine equal_rew_equal _ _ (λ n, _) t, { cases n; simp[concat, h] } }
-
-lemma equal_rew_iff {s₁ s₂ : ℕ → term L} (eqn : ∀ n, T ⊢ s₁ n =' s₂ n) (p : formula L) :
-  T ⊢ p.rew s₁ ⟷ p.rew s₂ :=
-begin
-  induction p generalizing T s₁ s₂,
-  case verum { simp[show (formula.verum : formula L) = ⊤, from rfl] },
-  case app : n p v { intros, simp[axiomatic_classical_logic'.iff_equiv],
-    suffices : ∀ (s₁ s₂ : ℕ → term L) (h : ∀ (n : ℕ), T ⊢ s₁ n =' s₂ n), T ⊢ formula.app p (λ i, (v i).rew s₁) ⟶ formula.app p (λ i, (v i).rew s₂),
-    { refine ⟨this _ _ eqn, this s₂ s₁ (λ x, eq_symm (eqn x))⟩ },
-    intros s₁ s₂ eqs,
-    have : T ⊢ ⋀ i, (v i).rew s₁ =' (v i).rew s₂,
-    { simp, intros i,refine equal_rew_equal _ _ eqs _ },
-    refine (predicate_ext' p _ _) ⨀ this },
-  case equal : t₁ t₂ { intros, simp[axiomatic_classical_logic'.iff_equiv],
-    refine ⟨deduction.mp _, deduction.mp _⟩,
-    { have lmm₁ : T+{t₁.rew s₁ =' t₂.rew s₁} ⊢ t₁.rew s₂ =' t₁.rew s₁,
-      { refine equal_rew_equal s₂ s₁ (λ n, eq_symm _) t₁, simp[eqn n] },
-      have lmm₂ : T+{t₁.rew s₁ =' t₂.rew s₁} ⊢ t₁.rew s₁ =' t₂.rew s₁, { simp },
-      have lmm₃ : T+{t₁.rew s₁ =' t₂.rew s₁} ⊢ t₂.rew s₁ =' t₂.rew s₂,
-      { refine equal_rew_equal s₁ s₂ (λ n, _) t₂, simp[eqn n]  },
-      refine eq_trans lmm₁ (eq_trans lmm₂ lmm₃) },
-    { have lmm₁ : T+{t₁.rew s₂ =' t₂.rew s₂} ⊢ t₁.rew s₁ =' t₁.rew s₂,
-      { refine equal_rew_equal s₁ s₂ (λ n, _) t₁, simp[eqn n] },
-      have lmm₂ : T+{t₁.rew s₂ =' t₂.rew s₂} ⊢ t₁.rew s₂ =' t₂.rew s₂, { simp },
-      have lmm₃ : T+{t₁.rew s₂ =' t₂.rew s₂} ⊢ t₂.rew s₂ =' t₂.rew s₁,
-      { refine equal_rew_equal s₂ s₁ (λ n, eq_symm _) t₂, simp[eqn n]  },
-      refine eq_trans lmm₁ (eq_trans lmm₂ lmm₃) } },
-  case imply : p q IH₁ IH₂
-  { intros, 
-    simp[axiomatic_classical_logic'.iff_equiv] at*, split,
-    { refine deduction.mp (deduction.mp _), 
-      have : T+{p.rew s₁ ⟶ q.rew s₁}+{p.rew s₂} ⊢ p.rew s₂, simp,
-      have : T+{p.rew s₁ ⟶ q.rew s₁}+{p.rew s₂} ⊢ p.rew s₁, from (by simp[IH₁ eqn]) ⨀ this,
-      have : T+{p.rew s₁ ⟶ q.rew s₁}+{p.rew s₂} ⊢ q.rew s₁,
-        from (show _ ⊢ p.rew s₁ ⟶ q.rew s₁, by simp) ⨀ this,
-      from (by simp[IH₂ eqn]) ⨀ this },
-    { refine deduction.mp (deduction.mp _),
-      have : T+{p.rew s₂ ⟶ q.rew s₂}+{p.rew s₁} ⊢ p.rew s₁, simp,
-      have : T+{p.rew s₂ ⟶ q.rew s₂}+{p.rew s₁} ⊢ p.rew s₂, from (by simp[IH₁ eqn]) ⨀ this,
-      have : T+{p.rew s₂ ⟶ q.rew s₂}+{p.rew s₁} ⊢ q.rew s₂,
-        from (show _ ⊢ p.rew s₂ ⟶ q.rew s₂, by simp) ⨀ this,
-      from (by simp[IH₂ eqn]) ⨀ this } },
-  case neg : p IH
-  { intros, simp[axiomatic_classical_logic'.iff_equiv] at*,
-    refine ⟨contrapose.mpr _, contrapose.mpr _⟩; simp[IH eqn] },
-  case fal : p IH
-  { intros, simp[axiomatic_classical_logic'.iff_equiv],
-    have := @IH (T^1) (s₁^1) (s₂^1)
-      (λ n, by { cases n; simp, exact sf_sf.mpr (eqn n) }),
-    simp[axiomatic_classical_logic'.iff_equiv] at this, 
-    refine ⟨univ_K _ _ ⨀ (generalize this.1), univ_K _ _ ⨀ (generalize this.2)⟩ }
-end
-
-lemma iff_of_eqs {s₁ s₂ : ℕ → term L} (eqn : ∀ n, T ⊢ s₁ n =' s₂ n) (p : formula L) :
-  T ⊢ p.rew s₁ ↔ T ⊢ p.rew s₂ :=
-⟨λ h, of_equiv_p h (equal_rew_iff eqn p), λ h, of_equiv_p h (equal_rew_iff (λ n, eq_symm $ eqn n) p)⟩
-
-lemma iff_rew_of_eq {t : term L} {n : ℕ} (eqn : T ⊢ #n =' t) (p : formula L) :
-  T ⊢ p ⟷ p.rew (λ x, if x = n then t else #x) :=
-begin
-  suffices : T ⊢ p.rew ı ⟷ p.rew (λ x, if x = n then t else #x), { simp*at* },
-  refine equal_rew_iff (λ x, _) _,
-  { by_cases C : x = n,
-    { rcases C with rfl, simp[ı, eqn] },
-    { simp[C] } }
-end
-
-lemma rew_of_eq (t : term L) (n : ℕ)
-  (eqn : T ⊢ #n =' t) {p : formula L} (h : T ⊢ p.rew (λ x, if x = n then t else #x)) :
-  T ⊢ p :=
-by have := iff_rew_of_eq eqn p; simp[iff_equiv] at this;
-   exact this.2 ⨀ h
-
-lemma specialize_iff {t : term L} (p : formula L) :
-  T ⊢ p.rew ı[0 ⇝ t] ⟷ ∀.((#0 =' t^1) ⟶ p) :=
-begin
-  simp[axiomatic_classical_logic'.iff_equiv], split,
-  { refine deduction.mp (generalize (deduction.mp _)),
-    simp[←sf_dsb],
-    have : (p.rew ı[0 ⇝ t])^1 = p.rew (λ x, if x = 0 then t^1 else #x),
-    { simp[formula.pow_rew_distrib, formula.pow_eq, formula.nested_rew],
-      congr, funext x, cases x; simp, refl },
-    rw this,
-    refine rew_of_eq (t^1) 0 (by simp) (by simp) },
-  { refine deduction.mp _,
-    have : T +{ ∀.((#0 =' t^1) ⟶ p) } ⊢ (t =' t) ⟶ formula.rew ı[0 ⇝ t] p,
-    { have := (show T +{ ∀.((#0 =' (t^1)) ⟶ p) } ⊢ ∀.((#0 =' (t^1)) ⟶ p), by simp) ⊚ t,
-      simp at this, exact this },
-    exact this ⨀ (by simp) }
-end
-
-lemma dummy_fal_quantifir (p) : T ⊢ p ⟷ ∀.p^1 :=
-by { have : T ⊢ ∀.(p^1) ⟶ (p^1).rew ı[0 ⇝ #0], from specialize #0, simp[*, axiomatic_classical_logic'.iff_equiv] at * }
-
-lemma dummy_fal_quantifir_iff {p : formula L} : T ⊢ ∀.(p^1) ↔ T ⊢ p :=
-by { have :=  (@dummy_fal_quantifir _ T p), simp[axiomatic_classical_logic'.iff_equiv] at this,  split,
-     { refine λ h, this ⨀ h },
-     { refine λ h, (by simp) ⨀ h } }
-
-lemma dummy_ex_quantifir (p) : T ⊢ p ⟷ ∃.p^1 :=
-by { simp[has_exists_quantifier.ex, formula.ex, axiomatic_classical_logic'.iff_equiv],
-     have : T ⊢ ∼p ⟷ ∀.(∼p) ^ 1, from dummy_fal_quantifir (∼p), simp[axiomatic_classical_logic'.iff_equiv] at this, 
-      split,
-     { refine contrapose.mp _, simp[this] },
-     { refine contrapose.mp _, simp[this] } }
-
-@[simp] lemma T_hyp_eliminate {p} : T ⊢ ⊤ ⟶ p ↔ T ⊢ p :=
-⟨λ h, by { have : T ⊢ ⊤, simp, exact h ⨀ this }, λ h, by simp[h]⟩
-
-lemma equiv_eq_of_equiv {t₁ u₁ t₂ u₂} (h₁ : T ⊢ t₁ =' u₁) (h₂ : T ⊢ t₂ =' u₂) : T ⊢ (t₁ =' t₂) ⟷ (u₁ =' u₂) :=
-by { simp[axiomatic_classical_logic'.iff_equiv],
-     refine ⟨deduction.mp _, deduction.mp  _⟩,
-     have lmm₁ : T+{t₁ =' t₂} ⊢ u₁ =' t₁, simp [eq_symm h₁],
-     have lmm₂ : T+{t₁ =' t₂} ⊢ t₁ =' t₂, simp,
-     have lmm₃ : T+{t₁ =' t₂} ⊢ t₂ =' u₂, simp [h₂],
-     refine eq_trans (eq_trans lmm₁ lmm₂) lmm₃,
-     have lmm₁ : T+{u₁ =' u₂} ⊢ t₁ =' u₁, simp [h₁],
-     have lmm₂ : T+{u₁ =' u₂} ⊢ u₁ =' u₂, simp,
-     have lmm₃ : T+{u₁ =' u₂} ⊢ u₂ =' t₂, simp [eq_symm h₂],
-     refine eq_trans (eq_trans lmm₁ lmm₂) lmm₃  }
-
-lemma eq_of_equiv {t₁ u₁ t₂ u₂} (h : T ⊢ t₁ =' u₁) (hp : T ⊢ t₁ =' t₂) (hq : T ⊢ u₁ =' u₂) : T ⊢ t₂ =' u₂ :=
-by { have := equiv_eq_of_equiv hp hq, simp[axiomatic_classical_logic'.iff_equiv] at this, exact this.1 ⨀ h, }
-
-lemma equiv_function_of_equiv {n} (f : L.fn n) {v₁ v₂ : finitary (term L) n} (h : ∀ i, T ⊢ v₁ i =' v₂ i) :
-  T ⊢ term.app f v₁ =' term.app f v₂ :=
-function_ext' f v₁ v₂ ⨀ (by simp[h])
-
-lemma equiv_predicate_of_equiv {n} (p : L.pr n) {v₁ v₂ : finitary (term L) n} (h : ∀ i, T ⊢ v₁ i =' v₂ i) :
-  T ⊢ formula.app p v₁ ⟷ formula.app p v₂ :=
-begin
-  simp[axiomatic_classical_logic'.iff_equiv],
-  refine ⟨(predicate_ext' p v₁ v₂) ⨀ (by simp[h]),
-  (predicate_ext' p v₂ v₁) ⨀ (by simp[λ i, eq_symm (h i)])⟩
-end
-
-lemma predicate_of_equiv {n} (p : L.pr n) {v₁ v₂ : finitary (term L) n} (h : T ⊢ formula.app p v₁) 
-  (hv : ∀ i, T ⊢ v₁ i =' v₂ i) : T ⊢ formula.app p v₂ :=
-by { have := equiv_predicate_of_equiv p hv, simp[axiomatic_classical_logic'.iff_equiv] at this, exact this.1 ⨀ h }
-
-lemma equiv_univ_of_equiv {p₁ p₂} (h : ⤊T ⊢ p₁ ⟷ p₂) : T ⊢ ∀.p₁ ⟷ ∀.p₂ :=
-by { simp[axiomatic_classical_logic'.iff_equiv] at h ⊢, refine ⟨univ_K _ _ ⨀ (generalize h.1), univ_K _ _ ⨀ (generalize h.2)⟩ }
-
-lemma univ_of_equiv {p₁ p₂} (h : T ⊢ ∀.p₁) (hp : ⤊T ⊢ p₁ ⟷ p₂) : T ⊢ ∀.p₂ :=
-(iff_equiv.mp (equiv_univ_of_equiv hp)).1 ⨀ h
-
-lemma equiv_univs_of_equiv {p₁ p₂} {n : ℕ} (h : T^n ⊢ p₁ ⟷ p₂) : T ⊢ (∀.[n] p₁) ⟷ (∀.[n] p₂) :=
-by { induction n with n IH generalizing p₁ p₂; simp, { exact h }, { simpa using IH (equiv_univ_of_equiv h) } }
-
-lemma equiv_ex_of_equiv {p₁ p₂} (h : ⤊T ⊢ p₁ ⟷ p₂) : T ⊢ ∃.p₁ ⟷ ∃.p₂ :=
-equiv_neg_of_equiv (equiv_univ_of_equiv (equiv_neg_of_equiv h))
-
-lemma ex_of_equiv {p₁ p₂} (h : T ⊢ ∃.p₁) (hp : ⤊T ⊢ p₁ ⟷ p₂) : T ⊢ ∃.p₂ :=
-(iff_equiv.mp (equiv_ex_of_equiv hp)).1 ⨀ h
-
-@[simp] protected lemma extend {T₀ T : Theory L} [T₀.extend T] {p : formula L} (h : T₀ ⊢ p) : T ⊢ p :=
-Theory.extend.le h
-
-lemma nfal_K (p q : formula L) (n) : T ⊢ (∀.[n] (p ⟶ q)) ⟶ (∀.[n] p) ⟶ ∀.[n] q :=
-begin
-  have eqn : ∀ p : formula L, (p.rew (λ x, ite (x < n) #x #(x + n))).rew (λ x, ite (x < n) #x #(x - n)) = p,
-  { intros p, simp[formula.nested_rew], 
-    have : (λ x, term.rew (λ (x : ℕ), ite (x < n) #x #(x - n)) (ite (x < n) #x #(x + n)) : ℕ → term L) = ı,
-    { funext x, by_cases C : x < n; simp[C] }, simp[this] },  
-  refine deduction.mp (deduction.mp (generalize_itr _)),
-  simp[pow_dsb],
-  have lmm₁ : (T^n) +{ (∀.[n] p ⟶ q)^n } +{ (∀.[n] p)^n } ⊢ p ⟶ q,
-  { have :  (T^n) +{ (∀.[n] p ⟶ q)^n } +{ (∀.[n] p)^n } ⊢ ∀.[n] p.rew (λ x, ite (x < n) #x #(x + n)) ⟶ q.rew (λ x, ite (x < n) #x #(x + n)),
-    { simp[show (∀.[n] p.rew (λ x, ite (x < n) #x #(x + n)) ⟶ q.rew (λ x, ite (x < n) #x #(x + n))) = (∀.[n] p ⟶ q)^n, by simp[formula.nfal_pow]] }, 
-    have := nfal_subst' this ı, simp[eqn] at this, exact this },
-  have lmm₂ : (T^n) +{ (∀.[n] p ⟶ q)^n } +{ (∀.[n] p)^n } ⊢ p,
-  { have : (T^n) +{ (∀.[n] p ⟶ q)^n } +{ (∀.[n] p)^n } ⊢ ∀.[n] p.rew (λ x, ite (x < n) #x #(x + n)),
-    { simp[show (∀.[n] p.rew (λ x, ite (x < n) #x #(x + n))) = (∀.[n] p)^n, by simp[formula.nfal_pow]] },
-    have := nfal_subst' this ı, simp[eqn] at this, exact this },
-  exact lmm₁ ⨀ lmm₂
-end
-
-lemma fal_complete_K (p q : formula L) : T ⊢ (∀.* (p ⟶ q)) ⟶ (∀.* p) ⟶ ∀.* q :=
-begin
-  refine (deduction.mp $ deduction.mp $ generalize_itr _), simp[pow_dsb],
-  have lmm₁ : (T ^ q.arity) +{ ∀.* (p ⟶ q) } +{ ∀.* p } ⊢ p ⟶ q,
-  { have : (T ^ q.arity) +{ ∀.* (p ⟶ q) } +{ ∀.* p } ⊢ ∀.* (p ⟶ q), by simp,
-    simpa using fal_complete_rew (p ⟶ q) ı ⨀ this },
-  have lmm₂ : (T ^ q.arity) +{ ∀.* (p ⟶ q) } +{ ∀.* p } ⊢ p,
-  { have : (T ^ q.arity) +{ ∀.* (p ⟶ q) } +{ ∀.* p } ⊢ ∀.* p, by simp,
-    simpa using fal_complete_rew p ı ⨀ this },
-  exact lmm₁ ⨀ lmm₂
-end
-
-lemma equiv_fal_complete_of_equiv {p₁ p₂ : formula L} (h : T^(max p₁.arity p₂.arity) ⊢ p₁ ⟷ p₂) :
-  T ⊢ (∀.* p₁) ⟷ (∀.* p₂) :=
-begin
-  simp[iff_equiv] at h ⊢, split,
-  { have : T ⊢ ∀.* (p₁ ⟶ p₂), from generalize_itr (by simp[h]),
-    exact fal_complete_K _ _ ⨀ this },
-  { have : T ⊢ ∀.* (p₂ ⟶ p₁), from generalize_itr (by simp[max_comm, h]),
-    exact fal_complete_K _ _ ⨀ this }
-end
-
-lemma nfal_rew {n} {p : formula L} (s : ℕ → term L) :
-  T ⊢ (∀.[n] p) ⟶ ∀.[n] p.rew (λ x, if x < n then s x else #x) :=
-begin
-  refine deduction.mp (generalize_itr _),
-  have : T +{ ∀.[n] p } ^ n ⊢ ∀.[n] p.rew (λ x, ite (x < n) #x #(x + n)),
-  { simp[pow_dsb, show (∀.[n] p.rew (λ x, ite (x < n) #x #(x + n))) = (∀.[n] p)^n, by simp[formula.nfal_pow]] },
-  have lmm : T +{ ∀.[n] p } ^ n ⊢ (p.rew (λ x, ite (x < n) #x #(x + n))).rew (λ x, ite (x < n) (s x) #(x - n)), from nfal_subst' this s,
-  simp[formula.nested_rew] at lmm,
-  have : (λ x, term.rew (λ x, ite (x < n) (s x) #(x - n)) (ite (x < n) #x #(x + n))) = (λ x, ite (x < n) (s x) #x),
-  { funext x, by_cases C : x < n; simp[C] },
-  simp[this] at lmm, exact lmm
-end
-
-@[simp] lemma fal_shift_equiv_self {p : formula L} : T ⊢ ∀.(p^1) ⟷ p :=
-begin
-  simp[axiomatic_classical_logic'.iff_equiv],
-  have : T ⊢ ∀.p^1 ⟶ (p^1).rew ı[0 ⇝ #0], from specialize #0,
-  simp at this, exact this
-end
-
-@[simp] lemma nfal_pow_equiv_self {p : formula L} {n : ℕ} : T ⊢ (∀.[n] p^n) ⟷ p :=
-begin
-  induction n with n IH,
-  { simp },
-  { simp[←nat.add_one],
-    have lmm : T ⊢ ∀.(∀.[n] p^n)^1 ⟷ p,
-    { have : T ⊢ ∀.(∀.[n] p^n)^1 ⟷ ∀.[n] p^n, { simp },
-      exact equiv_trans this IH },
-    have : (∀.[n] p^n)^1 = (∀.[n] p^(n + 1)), 
-    { simp[formula.pow_eq, formula.nested_rew, show ∀ x, x + (n + 1) = x + 1 + n, by omega] },
-    simp[this] at lmm, exact lmm }
-end
-
-variables (T)
-
-@[simp] lemma provable_Theory_refl : T ⊢ₜₕ T := λ p mem, by_axiom mem
-
-variables {T}
-
-lemma provable_Theory_weakening {U : Theory L} (h : T ⊆ U) : U ⊢ₜₕ T := λ p mem, by_axiom (h mem)
+instance : has_finite_character (formula L m) :=
+finite_character_of_finite_provable (formula L m) (λ T p, finite_character_aux)
 
 end provable
-
-variables {T : Theory L}
-
-namespace Theory
-variables {T₀ T₁ U₀ U₁ : Theory L}
-
-lemma le_of_ss : T₀ ⊆ T₁ → T₀ ≤ T₁ := λ hyp p h, weakening hyp h
-
-@[simp] lemma le_union_left : T₀ ≤ T₀ ∪ T₁ := le_of_ss (by simp)
-
-@[simp] lemma le_union_right : T₁ ≤ T₀ ∪ T₁ := le_of_ss (by simp)
-
-@[simp] lemma union_le_union (h₀ : T₀ ≤ U₀) (h₁ : T₁ ≤ U₁) : T₀ ∪ T₁ ≤ U₀ ∪ U₁ :=
-λ p b,
-begin
-  rcases provable.proof_conjunction_union b with ⟨P, Q, hP, hQ, b⟩,
-  have bP : U₀ ∪ U₁ ⊢ P.conjunction, from list_conjunction_provable (λ p hp, weakening (by simp[hp]) (h₀ (by_axiom (hP p hp)))),
-  have bQ : U₀ ∪ U₁ ⊢ Q.conjunction, from list_conjunction_provable (λ p hp, weakening (by simp[hp]) (h₁ (by_axiom (hQ p hp)))),
-  exact (weakening (by simp) b) ⨀ bP ⨀ bQ
-end
-
-section extend
-open logic.Theory
-
-def extend_of_inclusion {T₁ T₂ : Theory L} (ss : T₁ ⊆ T₂) : extend T₁ T₂ := ⟨le_of_ss ss⟩
-
-instance extend_ax₁ (p : formula L) : extend T (T +{ p }) := ⟨λ q h, by simp[h]⟩
-
-instance extend_ax₂ (p q : formula L) : extend T (T +{ p }+{ q }) := ⟨λ _ h, by simp[h]⟩
-
-instance extend_ax₃ (p q r : formula L) : extend T (T +{ p }+{ q }+{ r }) := ⟨λ _ h, by simp[h]⟩
-
-instance extend_ax₄ (p q r s : formula L) : extend T (T +{ p }+{ q }+{ r }+{ s }) := ⟨λ _ h, by simp[h]⟩
-
-instance extend_sf {T₁ T₂ : Theory L} [extend T₁ T₂] : extend (⤊T₁) (⤊T₂) :=
-⟨λ p h, by {
-  have : T₁ ⊢ ∀.p, from h.generalize,
-  have : T₂ ⊢ ∀.p, from this.extend,
-  have : ⤊T₂ ⊢ (∀.p)^1, from provable.sf_sf.mpr this,
-  simpa[formula.nested_rew] using this ⊚ #0 }⟩
-
-instance extend_pow (T₁ T₂ : Theory L) [ex : extend T₁ T₂] (k : ℕ) : extend (T₁^k) (T₂^k) :=
-by { induction k with k IH ; simp[Theory.sf_itr_succ], { exact ex }, { exactI fol.Theory.extend_sf } }
-
-instance extend_union_left (T₁ T₂ : Theory L) : extend T₁ (T₁ ∪ T₂) := Theory.extend_of_inclusion (by simp)
-
-instance extend_union_right (T₁ T₂ : Theory L) : extend T₂ (T₁ ∪ T₂) := Theory.extend_of_inclusion (by simp)
-
-instance extend_empty : extend ∅ T := Theory.extend_of_inclusion (by simp)
-
-instance extend_pow_of_closed (T₁ T₂ : Theory L) [closed_Theory T₁] [extend T₁ T₂] (k : ℕ) : extend T₁ (T₂^k) :=
-by simpa using Theory.extend_pow T₁ T₂ k
-
-instance union_extend_union [extend T₀ U₀] [extend T₁ U₁] : extend (T₀ ∪ T₁) (U₀ ∪ U₁) :=
-⟨union_le_union extend.le extend.le⟩
-
-end extend
-
-end Theory
-
-lemma provable.extend_pow {T₀ T : Theory L} [T₀.extend  T] [closed_Theory T₀] {p : formula L} (h : T₀ ⊢ p) (k : ℕ) :
-  T^k ⊢ p := by { have : T₀^k ⊢ p, by simp[h], exact this.extend }
-
-lemma proper_Theory_union (T₁ T₂ : Theory L) (h₁ : proper_Theory T₁) (h₂ : proper_Theory T₂) :
-  proper_at 0 (T₁ ∪ T₂) :=
-λ p s h, by { cases h,
-  { refine or.inl (proper_Theory.proper p s h) },
-  { refine or.inr (proper_Theory.proper p s h) } }
-
-def proper_schema (F : formula L → formula L) : Prop := ∃ i : ℕ, ∀ p s, (F p).rew s = F (p.rew (s^i))
-
-lemma proper_image_of_proper_schema (C : Theory L) [proper_Theory C]
-  {F : formula L → formula L} (h : proper_schema F) : proper_at 0 (F '' C) :=
-λ p s mem, begin
-    rcases mem with ⟨p, mem, rfl⟩,
-    rcases h with ⟨i, h⟩,
-    simp[h], refine ⟨p.rew (s^i), by simp[mem], rfl⟩
-end
-
-@[reducible] def prf (L : language) := Σ (T : Theory L) (p : formula L), T ⟹ p
-
-@[reducible] def prf.to_formula (b : prf L) : formula L := b.snd.fst
-
-@[reducible] def prf.to_proof (b : prf L) := b.snd.snd
-
-@[reducible] def proof.to_prf {p} (b : T ⟹ p) : prf L := ⟨T, p, b⟩
-
-namespace prf
-variables {T} {p : formula L} {b : T ⟹ p} {B : prf L}
-
-@[simp] lemma to_proof_to_prf : B.to_proof.to_prf = B := by { rcases B with ⟨T, p, b⟩, simp }
-
-@[simp] lemma to_prf_to_formula : b.to_prf.to_formula = p := rfl
-
-@[simp] lemma to_prf_to_proof : b.to_prf.to_proof = b := rfl
-
-end prf
-
-namespace proof
-variables {T} {p : formula L}
-
-inductive subproof : prf L → prf L → Prop
-| mdp₁    : ∀ {T : Theory L} {p q : formula L} {b₁ : T ⟹ (p ⟶ q)} {b₂ : T ⟹ p}, subproof ⟨T, p ⟶ q, b₁⟩ ⟨T, q, mdp b₁ b₂⟩ 
-| mdp₂    : ∀ {T : Theory L} {p q : formula L} {b₁ : T ⟹ (p ⟶ q)} {b₂ : T ⟹ p}, subproof ⟨T, p, b₂⟩ ⟨T, q, mdp b₁ b₂⟩
-| generalize : ∀ {T : Theory L} {p : formula L} {b : ⤊T ⟹ p}, subproof ⟨⤊T, p, b⟩ ⟨T, ∀.p, b.generalize⟩ 
-
-@[simp] def complexity : Π {T : Theory L} {p : formula L} (b : T ⟹ p), ℕ
-| T p (generalize b)            := b.complexity + 1
-| T p (mdp b₁ b₂)               := max b₁.complexity b₂.complexity + 1
-| T p (by_axiom h)              := 0
-| T _ verum                     := 0
-| T _ (@imply₁ _ _ p q)         := 0
-| T _ (@imply₂ _ _ p q r)       := 0
-| T _ (@contraposition _ _ p q) := 0
-| T _ (@specialize _ _ p t)     := 0
-| T _ (@univ_K _ _ p q)         := 0
-| T _ (@dummy_univ _ _ p)       := 0
-| T _ (@eq_reflexivity _ _)     := 0
-| T _ eq_symmetry               := 0
-| T _ eq_transitivity           := 0
-| T _ (@function_ext _ _ _ f)   := 0
-| T _ (@predicate_ext _ _ _ r)  := 0
-
-instance : wf_lt (prf L) :=
-{ prelt := subproof,
-  wt := λ b, b.snd.snd.complexity,
-  mono' := λ b₁ b₂ h, by { induction h; try { simp },
-  case mdp₁ : T p q b₁ b₂ { exact nat.lt_succ_iff.mpr (le_max_left b₁.complexity b₂.complexity) },
-  case mdp₂ : T p q b₁ b₂ { exact nat.lt_succ_iff.mpr (le_max_right b₁.complexity b₂.complexity) } } }
-
-def le {T₁ T₂ : Theory L} {p₁ p₂ : formula L} (b₁ : T₁ ⟹ p₁) (b₂ : T₂ ⟹ p₂) : Prop := b₁.to_prf ≤ b₂.to_prf
-
-def lt {T₁ T₂ : Theory L} {p₁ p₂ : formula L} (b₁ : T₁ ⟹ p₁) (b₂ : T₂ ⟹ p₂) : Prop := b₁.to_prf < b₂.to_prf
-
-def fn_symbols {p} (b : T ⟹ p) : set (Σ n, L.fn n) :=
-  let B : set (prf L) := {c | c < b.to_prf},
-      B' : set (formula L) := prf.to_formula '' B in ⋃₀ (formula.fn_symbols '' B')
-
-section
-variables {T₁ T₂ : Theory L} {p₁ p₂ : formula L}
-
-@[simp] lemma lt_generalize_iff {b₁ : prf L} {b₂ : ⤊T₂ ⟹ p₂} : b₁ < b₂.generalize.to_prf ↔ b₁ ≤ b₂.to_prf :=
-by { simp[lt, le, wf_lt.lt_iff], split,
-     { rintros ⟨T, p, b, prelt, le⟩, rcases prelt, exact le },
-     { intros le, refine ⟨⤊T₂, p₂, b₂, subproof.generalize, le⟩ } }
-
-@[simp] lemma lt_mdp_iff {q₂ : formula L} {b₁ : prf L} {b₂₁ : T₂ ⟹ p₂ ⟶ q₂} {b₂₂ : T₂ ⟹ p₂} :
-  b₁ < (mdp b₂₁ b₂₂).to_prf ↔ b₁ ≤ b₂₁.to_prf ∨ b₁ ≤ b₂₂.to_prf :=
-by { simp[lt, le, wf_lt.lt_iff], split,
-     { rintros ⟨T, p, b, prelt, le⟩, rcases prelt, { exact or.inl le }, { exact or.inr le } },
-     { rintros (le | le), refine ⟨T₂, p₂ ⟶ q₂, b₂₁, subproof.mdp₁, le⟩, refine ⟨T₂, p₂, b₂₂, subproof.mdp₂, le⟩ } }
-
-end
-
-@[simp] lemma wt_eq_complexity (T) (p) (b) : wf_lt.wt (⟨T, p, b⟩ : prf L) = complexity b :=
-by refl
-
-lemma prelt_finite (b : prf L) : set.finite {c | subproof c b} :=
-begin
-  have of_eq_empty : ∀ s : set (prf L), s = ∅ → s.finite,
-  { rintros _ rfl, simp }, 
-  rcases b with ⟨T, p, b⟩,
-  induction b;
-  try { refine of_eq_empty _
-    (by { ext c, simp, intros h, 
-      have : wf_lt.wt c < wf_lt.wt _, from wf_lt.lt_mono (wf_lt.lt_of_prelt (show wf_lt.prelt c ⟨_, _, _⟩, from h)),
-      simp at this, contradiction }) },
-  case generalize : T p b
-  { have : {c : prf L | subproof c ⟨T, ⟨∀.p, b.generalize⟩⟩} = {b.to_prf},
-    { ext c, simp, split,
-      { intros h, rcases h, refl }, { rintros rfl, exact subproof.generalize } },
-    simp[this] },
-  case mdp : T p q b₁ b₂
-  { have : {c : prf L | subproof c ⟨T, ⟨q, b₁.mdp b₂⟩⟩} = {b₁.to_prf, b₂.to_prf},
-    { ext c, simp, split,
-      { intros h, rcases h, refine or.inl rfl, refine or.inr rfl },
-      { rintros (rfl | rfl), refine subproof.mdp₁, refine subproof.mdp₂ } },
-    simp[this] }
-end
-
-lemma le_finite (b : prf L) : set.finite {b' | b' ≤ b} :=
-wf_lt.le_finite (show ∀ (a : prf L), {b : prf L | wf_lt.prelt b a}.finite, from prelt_finite) b
-
-def formula_mem_proof (p : formula L) {T : Theory.{u} L} {q : formula.{u} L} (b : T ⟹ q) : Prop := ∃ (b' ≤ b.to_prf),p ≤ b'.to_formula
-
-infix ` ∈ᶠ `:50 := formula_mem_proof
-
-@[simp] lemma formula_mem_self {T : Theory L} {p : formula L} (b : T ⟹ p) : p ∈ᶠ b := ⟨b.to_prf, by simp⟩
-
-def term_mem_proof (t : term L) {T : Theory.{u} L} {p : formula.{u} L} (b : T ⟹ p) : Prop := ∃ (b' ≤ b.to_prf), t ∈ b'.to_formula
-
-infix ` ∈ᵗ `:50 := term_mem_proof
-
-section
-variables {T} {p} {b : T ⟹ p} {T₁ T₂ : Theory L} {p₁ p₂ : formula L} {b₁ : T₁ ⟹ p₁} {b₂ : T₂ ⟹ p₂} {B : prf L}
-
-lemma term_mem_proof_def {t : term L} :
-  t ∈ᵗ b ↔ ∃ b' ≤ b.to_prf, t ∈ b'.to_formula := by refl
-
-lemma mem_trans {t : term L} {q : formula L}
-  (ht : t ∈ q) (hq : q ∈ᶠ b) : t ∈ᵗ b :=
-by { rcases hq with ⟨b', hb', hq⟩, refine ⟨b', hb', formula.mem_of_formula_le_mem ht hq⟩ }
-
-@[simp] lemma mem_self (B : prf L) : B.to_formula ∈ᶠ B.to_proof := ⟨B, by simp, by simp⟩
-
-lemma formula_mem_proof.mem_of_mem_of_le {p'} (mem : p' ∈ᶠ b) (le : b.to_prf ≤ B) : p' ∈ᶠ B.to_proof :=
-by { rcases mem with ⟨b', le_b', ge_b'⟩,
-     refine ⟨b', by { simp, exact le_trans le_b' le }, ge_b'⟩ }
-
-lemma term_mem_proof.mem_of_mem_of_le {t'} (mem : t' ∈ᵗ b) (le : b.to_prf ≤ B) : t' ∈ᵗ B.to_proof :=
-by { rcases mem with ⟨b', le_b', ge_b'⟩,
-     refine ⟨b', by { simp, exact le_trans le_b' le }, ge_b'⟩ }
-
-lemma formula_mem_proof.mem_of_le_of_mem {p' q} (le : q ≤ p') (mem : p' ∈ᶠ b) : q ∈ᶠ b :=
-by { rcases mem with ⟨b', le_b', ge_b'⟩, refine ⟨b', le_b', le_trans le ge_b'⟩ }
-
-lemma term_mem_proof.mem_of_le_of_mem {t u} (le : u ≤ t) (mem : t ∈ᵗ b) : u ∈ᵗ b :=
-by { rcases mem with ⟨b', le_b', ge_b'⟩, refine ⟨b', le_b', formula.mem_of_term_le_mem ge_b' le⟩ }
-
-@[simp] lemma term_mem_generalize_iff {b : ⤊T ⟹ p} {t : term L} : t ∈ᵗ b.generalize ↔ t ∈ᵗ b :=
-⟨by { rintros ⟨b', le, mem⟩,
-      have : b' < b.generalize.to_prf ∨ b' = b.generalize.to_prf, exact lt_or_eq_of_le le,
-      rcases this with (lt | rfl),
-      { simp at lt, 
-        have : b'.to_formula ∈ᶠ b, from (mem_self b').mem_of_mem_of_le (show b'.to_proof.to_prf ≤ b.to_prf, by simp[lt]),
-        refine mem_trans mem this },
-      { simp at mem, refine mem_trans mem (by simp) } },
- λ h, h.mem_of_mem_of_le (show b.to_prf ≤ b.generalize.to_prf, from le_of_lt (by simp))⟩ 
-
-@[simp] lemma term_mem_mdp_iff {p q} {b₁ : T ⟹ p ⟶ q} {b₂ : T ⟹ p} {t} : t ∈ᵗ (b₁.mdp b₂) ↔ t ∈ᵗ b₁ ∨ t ∈ᵗ b₂ :=
-⟨by { rintros ⟨b', le, mem⟩,
-      have : b' < (b₁.mdp b₂).to_prf ∨ b' = (b₁.mdp b₂).to_prf, exact lt_or_eq_of_le le,
-      rcases this with (lt | rfl),
-      { simp at lt, rcases lt, 
-        { have : b'.to_formula ∈ᶠ b₁, from (mem_self b').mem_of_mem_of_le (show b'.to_proof.to_prf ≤ b₁.to_prf, by simp[lt]),
-          refine or.inl (mem_trans mem this) },
-        { have : b'.to_formula ∈ᶠ b₂, from (mem_self b').mem_of_mem_of_le (show b'.to_proof.to_prf ≤ b₂.to_prf, by simp[lt]),
-          refine or.inr (mem_trans mem this) }, },
-      { simp at mem, refine or.inl (mem_trans mem
-          (formula_mem_proof.mem_of_le_of_mem (show q ≤ p ⟶ q, from le_of_lt (by simp)) (by simp))) } },
- λ h, by { rcases h with (h | h),
-           { exact h.mem_of_mem_of_le (show b₁.to_prf ≤ (b₁.mdp b₂).to_prf, from le_of_lt (by simp)) },
-           { exact h.mem_of_mem_of_le (show b₂.to_prf ≤ (b₁.mdp b₂).to_prf, from le_of_lt (by simp)) } }⟩ 
-
-private lemma not_mem_of (b : T ⟹ p) (h : b.complexity = 0) (t : term L) : t ∈ᵗ b ↔ t ∈ p :=
-⟨by { rintros ⟨b', le, mem⟩, have : b' < b.to_prf ∨ b' = b.to_prf, exact lt_or_eq_of_le le,
-      rcases this with (lt | rfl),
-      { have : wf_lt.wt b' < wf_lt.wt b.to_prf, from wf_lt.lt_mono lt,
-        simp[h] at this, contradiction },
-      { simp at mem, exact mem } },
- by { intros mem, refine ⟨b.to_prf, by simp, by simp[mem]⟩ }⟩
-
-
-@[simp] lemma term_mem_by_axiom_iff {h : p ∈ T} {t} : t ∈ᵗ by_axiom h ↔ t ∈ p := not_mem_of _ (by simp) _
-
-@[simp] lemma term_mem_verum_iff {t} : ¬t ∈ᵗ (verum : T ⟹ ⊤) := by { have := not_mem_of (verum : T ⟹ ⊤) (by simp) t, simp at this, exact this }
-
-@[simp] lemma term_mem_imply₁_iff {p q : formula L} {t} : t ∈ᵗ (@imply₁ _ T p q) ↔ t ∈ p ∨ t ∈ q :=
-by { have := not_mem_of (@imply₁ _ T p q) (by simp) t, simp at this, simp[this], tauto }
-
-@[simp] lemma term_mem_imply₂_iff {p q r : formula L} {t} : t ∈ᵗ (@imply₂ _ T p q r) ↔ t ∈ p ∨ t ∈ q ∨ t ∈ r :=
-by { have := not_mem_of (@imply₂ _ T p q r) (by simp) t, simp at this, simp[this], tauto }
-
-@[simp] lemma term_mem_contraposition_iff {p q : formula L} {t} :
-  t ∈ᵗ (@contraposition _ T p q) ↔ t ∈ p ∨ t ∈ q :=
-by { have := not_mem_of (@contraposition _ T p q) (by simp) t, simp at this, simp[this], tauto }
-
-@[simp] lemma term_mem_specialize_iff {p : formula L} {t₀ t} :
-  t ∈ᵗ (@specialize _ T p t₀) ↔ t ∈ p ∨ t ∈ formula.rew ı[0 ⇝ t₀] p :=
-by { have := not_mem_of (@specialize _ T p t₀) (by simp) t, simp at this, simp[this] }
-
-@[simp] lemma term_mem_univ_K_iff {p q : formula L} {t} :
-  t ∈ᵗ (@univ_K _ T p q) ↔ t ∈ p ∨ t ∈ q :=
-by { have := not_mem_of (@univ_K _ T p q) (by simp) t, simp at this, simp[this] }
-
-@[simp] lemma term_mem_dummy_univ_iff {p : formula L} {t} :
-  t ∈ᵗ (@dummy_univ _ T p) ↔ t ∈ p ∨ t ∈ p^1 :=
-by { have := not_mem_of (@dummy_univ _ T p) (by simp) t, simp at this, simp[this] }
-
-variables (b)
-
-lemma term_mem_finite {T : Theory L} {p : formula L} (b : T ⟹ p) : set.finite {t | t ∈ᵗ b} :=
-begin
-  let s := ⋃ b' ∈ {b' | b' ≤ b.to_prf}, {t | t ∈ b'.to_formula},
-  have : {t | t ∈ᵗ b} = s,
-  { ext t, simp[s, term_mem_proof_def] },
-  simp[this],
-  refine set.finite.bUnion (le_finite b.to_prf) (λ b' _, b'.to_formula.mem_finite) 
-end
-
-end
-
-end proof
-
-namespace Theory
-open provable
-variables {T} {U : Theory L}
-
-lemma le_iff_mem_provable :
-  T ≤ U ↔ ∀ p ∈ T, U ⊢ p :=
-⟨λ h p mem, h (by_axiom mem), by { 
-  suffices : ∀ (T : Theory L) (k : ℕ) (p : formula L) (b : T^k ⊢ p) (h : ∀ p ∈ T, U ⊢ p), U^k ⊢ p,
-  { intros h p b, exact this T 0 p b h },
-  intros T k p b,
-  refine rec'_on b _ _ _ _ _ _ _ _ _ _ _ _ _ _ _; try { simp },
-  { intros i p b IH h, exact generalize (IH h) },
-  { intros i p q b₁ b₂ IH_b₁ IH_b₂ h, exact IH_b₁ h ⨀ IH_b₂ h },
-  { intros i p mem h, simp[Theory_sf_itr_eq] at mem, rcases mem with ⟨p, mem, rfl⟩,
-    exact sf_itr_sf_itr.mpr (h p mem) } }⟩
-
-end Theory
 
 end fol
